added result on cases that do not correspond to the tag. Started adding result for tag case.

theories/iris/logrel/instr/typing/case.v
@@ -14,15 +14,40 @@ Section case.
   Variable sr : store_runtime.
   Variable mr : module_runtime.
 
-  Lemma compat_case_block_fail F wt wt_save tag_idx (tag i : nat) f wl_others wl_ret es_drop_i es_get_locals_i es_case_i B R wl wl_save τ_res val_idxs case_i_val_idxs case_i_sum_locals (vs_res vs_payload case_i_vs_payload : list value) :
+  (* TODO: this should probably be a definition in the compiler. *)
+  Definition compile_cases :=
+    (fix compile_cases
+    (fe : function_env) (ess : list (list instruction)) {struct ess} : list (codegen ()) :=
+      match ess with
+      | [] => []
+      | es :: ess' =>
+          mapM_ (compile_instr mr fe) es :: compile_cases fe ess'
+      end).
+
+  Lemma compile_cases_length fe ess :
+    length ess = length $ compile_cases fe ess.
+  Proof.
+    induction ess as [|? ? IH]; [done | simpl; rewrite IH; done].
+  Qed.
+
+  Lemma compile_cases_app fe ess1 ess2 :
+    (fix compile_cases fe ess := match ess with
+     | [] => [] | es :: ess' => mapM_ (compile_instr mr fe) es :: compile_cases fe ess'
+     end) fe (ess1 ++ ess2) =
+    (fix compile_cases fe ess := match ess with
+     | [] => [] | es :: ess' => mapM_ (compile_instr mr fe) es :: compile_cases fe ess'
+     end) fe ess1 ++
+    (fix compile_cases fe ess := match ess with
+     | [] => [] | es :: ess' => mapM_ (compile_instr mr fe) es :: compile_cases fe ess'
+     end) fe ess2.
+  Proof.
+    induction ess1; simpl; [done | by rewrite IHess1].
+  Qed.
+
+
+  Lemma compat_case_block_fail F tag_idx (tag i : nat) f wl_ret es_drop_i es_get_locals_i es_case_i B R τ_res (vs_res : list value) :
     let fe := fe_of_context F in
     f_locs f !! tag_idx = Some (VAL_int32 (Wasm_int.Int32.repr tag)) ->
-    run_codegen (get_locals_w case_i_val_idxs) (wt ++ wt_save)
-      (wl ++ wl_save ++ [prelude.W.T_i32] ++ wl_others) = inr ((), [], [], es_get_locals_i) ->
-    run_codegen (drop_consts wl_ret) (wt ++ wt_save)
-      (wl ++ wl_save ++ [prelude.W.T_i32] ++ wl_others) = inr ((), [], [], es_drop_i) ->
-    util.nths_error val_idxs case_i_sum_locals = Some case_i_val_idxs ->
-    util.nths_error vs_payload case_i_sum_locals = Some case_i_vs_payload ->
     prelude.translate_type (fe_type_vars fe) τ_res = Some wl_ret ->
     tag ≠ i ->
     (tag < Wasm_int.Int32.modulus)%Z ->
@@ -42,7 +67,7 @@ Section case.
         UNDER B; R
         {{ fr'; vs', ⌜fr' = f⌝ ∗ ⌜vs' = vs_res⌝ }}.
   Proof.
-    intros fe Hlookup_saved_and_tag Hget_locals_i Hdrop_consts_i Hnerr_val_idxs Hnerr_payload_ci Htranslate_type_fe Hneq Htag_lt Hi_lt Hvs_res_length.
+    intros fe Hlookup_saved_and_tag Htranslate_type_fe Hneq Htag_lt Hi_lt Hvs_res_length.
     iIntros "Hfr Hrun".
 
     iApply (cwp_block with "[$] [$]"); auto.
@@ -110,7 +135,126 @@ Section case.
   Qed.
 
 
-  (* TODO: should probably be written using run_codegen somehow *)
+  Lemma compat_case_blocks_fail F wt wt' (tag_idx : nat) tag wl_ret wl wl' ρs_sum
+    val_localidxs vs_res
+    (ess : list (list instruction)) es_fail_cases (start : nat) fr B R τ_res :
+    let fe := fe_of_context F in
+    let tag_localidx := Mk_localidx tag_idx in
+    (tag < start ∨ tag ≥ start + length ess) ->
+    f_locs fr !! tag_idx = Some (VAL_int32 (Wasm_int.Int32.repr tag)) ->
+    prelude.translate_type (fe_type_vars fe) τ_res = Some wl_ret ->
+    (tag < Wasm_int.Int32.modulus)%Z ->
+    (length ρs_sum <= Wasm_int.Int32.modulus)%Z ->
+    (length ess <= length ρs_sum)%Z ->
+    length vs_res = length wl_ret ->
+    run_codegen
+      (case_blocks_blocks start tag_localidx wl_ret
+         (map (λ c i,
+            try_option EFail (ρs_sum !! i)
+            ≫= λ ρ, try_option EFail (inject_sum_rep EmptyEnv ρs_sum ρ)
+            ≫= λ ixs', (try_option EFail (nths_error val_localidxs ixs')
+                         ≫= get_locals_w)
+            ≫= λ _, c)
+            (compile_cases fe ess)))
+      wt wl =
+    inr ((), wt', wl', es_fail_cases) ->
+    ⊢
+    ↪[frame]fr -∗
+    ↪[RUN] -∗
+    CWP to_consts vs_res ++ es_fail_cases
+      UNDER B; R
+      {{ fr'; vs', ⌜fr' = fr⌝ ∗ ⌜vs' = vs_res⌝ }}.
+  Proof.
+    revert start wt wl wt' wl' es_fail_cases.
+    induction ess as [| es_hd ess IH]; intros start wt wl wt' wl' es_fail_cases fe tag_localidx
+        Hrange Htag_lookup Htranslate Htag_lt Hlen_lt Hlen_le Hvs_len Hcg.
+    - (* base case: no blocks *)
+      simpl in Hcg.
+      inv_cg_ret Hcg; subst.
+      iIntros "Hfr Hrun".
+      rewrite app_nil_r.
+      iApply (cwp_val with "[$] [$]").
+      1: apply has_values_to_consts.
+      done.
+    - (* inductive case *)
+      simpl compile_cases in Hcg.
+      rewrite map_cons in Hcg.
+      change (run_codegen
+        (case_block tag_localidx wl_ret
+           (λ i, try_option EFail (ρs_sum !! i)
+                 ≫= λ ρ, try_option EFail (inject_sum_rep EmptyEnv ρs_sum ρ)
+                 ≫= λ ixs', (try_option EFail (nths_error val_localidxs ixs')
+                              ≫= get_locals_w)
+                 ≫= λ _, mapM_ (compile_instr mr fe) es_hd) start ;;
+         case_blocks_blocks (S start) tag_localidx wl_ret
+           (map (λ c i,
+              try_option EFail (ρs_sum !! i)
+              ≫= λ ρ, try_option EFail (inject_sum_rep EmptyEnv ρs_sum ρ)
+              ≫= λ ixs', (try_option EFail (nths_error val_localidxs ixs')
+                           ≫= get_locals_w)
+              ≫= λ _, c)
+              (compile_cases fe ess)))
+        wt wl = inr ((), wt', wl', es_fail_cases)) in Hcg.
+      apply run_codegen_bind_dist in Hcg as
+        (x1 & wt1 & wt2 & wl1 & wl2 & es1 & es2 & Hcg_hd & Hcg_tl & -> & -> & ->).
+
+      (* Case es_i *)
+      inv_cg_bind Hcg_hd ?pair ?wt ?wt ?wl ?wl ?es ?es Hcase_es_i Hcase_es_i_block.
+      destruct pair, u.
+      inv_cg_emit Hcase_es_i_block; subst.
+      apply run_codegen_capture in Hcase_es_i as [Hcase_es_i ->].
+
+      inv_cg_bind Hcase_es_i [] ?wt ?wt ?wl ?wl ?es ?es Hget_tag Hcase_es_i.
+      inv_cg_emit Hget_tag; subst.
+
+      inv_cg_bind Hcase_es_i [] ?wt ?wt ?wl ?wl ?es ?es Htag0 Hcase_es_i.
+      inv_cg_emit Htag0; subst.
+
+      inv_cg_bind Hcase_es_i [] ?wt ?wt ?wl ?wl ?es ?es Hcompare_tag Hcase_es_i.
+      inv_cg_emit Hcompare_tag; subst.
+
+      inv_cg_bind Hcase_es_i [] ?wt ?wt ?wl ?wl ?es ?es Hbr_case Hcase_es_i.
+      inv_cg_emit Hbr_case; subst.
+
+      inv_cg_bind Hcase_es_i [] ?wt ?wt ?wl ?wl es_drop_i ?es Hdrop_consts_i Hcase_es_i.
+      apply run_codegen_drop_consts in Hdrop_consts_i as H.
+      destruct H as (_ & -> & -> & _).
+
+      inv_cg_bind Hcase_es_i ρ_casei ?wt ?wt ?wl ?wl ?es ?es Hlookup Hcase_es_i.
+      inv_cg_try_option Hlookup; subst.
+
+      inv_cg_bind Hcase_es_i case_i_sum_locals ?wt ?wt ?wl ?wl ?es ?es Hinject Hcase_es_i.
+      inv_cg_try_option Hinject; subst.
+
+      inv_cg_bind Hcase_es_i [] ?wt wt_case_i ?wl wl_case_i ?es es_case_i Hget_locals_i Hcase_es_i.
+      inv_cg_bind Hget_locals_i case_i_val_idxs ?wt wt_get_locals_i ?wl wl_get_locals_i ?es es_get_locals_i Hnths_error Hget_locals_i.
+      inv_cg_try_option Hnths_error; subst.
+
+      destruct (run_codegen_get_locals _ _ _ _ _ _ _ Hget_locals_i) as ([] & -> & ->).
+
+      (* clean up *)
+      clear_nils.
+      simplify_eq.
+
+      iIntros "Hfr Hrun".
+      rewrite app_assoc.
+      iApply (cwp_seq with "[Hfr Hrun]").
+      {
+        iApply (compat_case_block_fail with "[$] [$]"); try done.
+        - destruct Hrange as [Hlt | Hge]; simpl in *; lia.
+        - destruct Hrange as [Hlt | Hge]; simpl in *.
+          + apply lookup_lt_Some in Heq_some. lia.
+          + lia.
+      }
+      iIntros (?fr w) "(-> & ->) Hfr Hrun".
+      iApply (IH (S start) with "[$] [$]"); try done.
+      + destruct Hrange as [Hlt | Hge]; simpl in *.
+        * left. lia.
+        * right. lia.
+      + simpl in Hlen_le. lia.
+  Qed.
+
+
   Lemma compat_case_block_success M F L wt wt_save wt_cases wt_others wtf tag_idx (tag i : nat) fr_saved_and_tag wl_ret lmask es_drop_i es_get_locals_i es_case_i B R se L' wl wl_save wl_others wl_cases wlf (τs: list type) τ_i τ_tag τ_res os_payload case_i_os_payload val_localidxs case_i_val_idxs case_i_sum_locals (vs_res vs_payload case_i_vs_payload : list value) θ :
     let F' := F <| fc_labels ::= cons ([τ_res], L') |> in
     let fe := fe_of_context F in
@@ -311,1008 +455,1093 @@ Section case.
     by iFrame.
   Admitted.
 
-
-
-  Lemma compat_binary_case M F L L' wt wt' wtf wl wl' wlf es' ess es1 es2 τs τ1 τ2 τs' κ :
-    ess = [es1; es2] ->
-    τs = [τ1; τ2] ->
+Lemma compat_case_block_success_cg M F L wt wt_case_tag wtf tag_idx (tag : nat)
+    wl_ret lmask B R se L' wl wl_case_tag wlf
+    (τs: list type) τ_tag τ_res os_tag val_localidxs vs_payload
+    ρs_sum fr_saved_and_tag θ
+    os_payload
+    es_tag_cg
+    (ess_pre : list (list instruction))
+    (es_tag : list instruction) :
+    let F' := F <| fc_labels ::= cons ([τ_res], L') |> in
     let fe := fe_of_context F in
-    let WT := wt ++ wt' ++ wtf in
-    let WL := wl ++ wl' ++ wlf in
-    let lmask := wlmask fe wl in
-    let F' := F <| fc_labels ::= cons (τs', L') |> in
-    let ψ := InstrT [SumT κ τs] τs' in
-    Forall2
-      (fun τ es =>
-         (forall wt wt' wtf wl wl' wlf es',
-            let fe' := fe_of_context F' in
-            let WT := wt ++ wt' ++ wtf in
-            let WL := wl ++ wl' ++ wlf in
-            let lmask := wlmask fe' wl in
-            run_codegen (compile_instrs mr fe' es) wt wl = inr ((), wt', wl', es') ->
-            ⊢ have_instr_type_sem rti sr mr M F' L WT WL lmask es' (InstrT [τ] τs') L'))
-      τs ess ->
-    has_instruction_type_ok F ψ L' ->
-    run_codegen (compile_instr mr fe (ICase ψ L' ess)) wt wl = inr ((), wt', wl', es') ->
-    ⊢ have_instr_type_sem rti sr mr M F L WT WL lmask es' ψ L'.
+    let tag_localidx := Mk_localidx tag_idx in
+    f_locs fr_saved_and_tag !! tag_idx = Some (VAL_int32 (Wasm_int.Int32.repr tag)) ->
+    prelude.translate_type (fe_type_vars fe) τ_res = Some wl_ret ->
+    τs !! tag = Some τ_tag ->
+    length ess_pre = tag ->
+    sem_env_interp F se ->
+    run_codegen
+      (case_block tag_localidx wl_ret
+         (λ i,
+            try_option EFail (ρs_sum !! i)
+            ≫= λ ρ, try_option EFail (inject_sum_rep EmptyEnv ρs_sum ρ)
+            ≫= λ ixs', (try_option EFail (nths_error val_localidxs ixs')
+                         ≫= get_locals_w)
+            ≫= λ _, mapM_ (compile_instr mr fe) es_tag)
+         (length ess_pre))
+      wt wl =
+    inr ((), wt_case_tag, wl_case_tag, es_tag_cg) ->
+    ⊢
+    have_instr_type_sem rti sr mr M F' L
+          (wt ++ wt_case_tag ++ wtf)
+          (wl ++ wl_case_tag ++ wlf)
+          lmask es_tag_cg (InstrT [τ_tag] [τ_res]) L' -∗
+    instance_interp rti sr mr M (wt ++ wt_case_tag ++ wtf) fr_saved_and_tag.(f_inst) -∗
+      labels_interp rti sr se fr_saved_and_tag (wl ++ wl_case_tag ++ wlf)
+          lmask (fc_labels F) B -∗
+    return_interp rti sr se (fc_return F) R -∗
+    rt_token rti sr θ -∗
+    ▷ value_interp rti sr se τ_tag (SAtoms os_tag) -∗
+    atoms_interp os_payload vs_payload -∗
+    frame_interp rti sr se L (wl ++ wl_case_tag ++ wlf) fr_saved_and_tag -∗
+    ↪[frame]fr_saved_and_tag -∗
+    ↪[RUN] -∗
+      CWP to_consts (map default_of_value_type wl_ret) ++ es_tag_cg
+        UNDER B; R
+        {{ fr'; vs',
+              ⌜length vs' = length wl_ret⌝ ∗
+              ⌜frame_rel lmask fr_saved_and_tag fr'⌝ ∗
+              frame_interp rti sr se L' (wl ++ wl_case_tag ++ wlf) fr' ∗
+              ∃ (os' : leibnizO (list atom)) (θ : address_map),
+               values_interp rti sr se [τ_res] os' ∗ atoms_interp os' vs' ∗
+               rt_token rti sr θ
+        }}.
 Proof.
-    intros -> -> fe WT WL lmask F' Ψ Hforall Hok Hcg.
-    set (τs := [τ1; τ2]).
-    rewrite Forall2_cons_iff in Hforall.
-    destruct Hforall as [Hes1 H2].
-    rewrite Forall2_cons_iff in H2.
-    destruct H2 as [Hes2 _].
-    subst Ψ.
-    cbn [compile_instr] in Hcg.
-    destruct κ as [ ρ rf | ]; last inversion Hcg.
-    destruct ρ  as [ | ρs_sum | | ]; try done.
-    destruct τs' as [ | τ_res τs' ]; first done.
-    destruct τs'; last done.
+  intros F' fe tag_localidx Hlookup_saved_and_tag Htranslate_type_fe Ht_lookup_tag Heq Hsem Hcg_tag.
+    iIntros "Hsem_es_tag #Hinst #Hlabels #Hreturn Hrt Hvalue_interp_os_tag Hatoms_interp_payload Hframe_saved_and_tag Hfr Hrun".
 
-    inv_cg_bind Hcg wl_ret ?wt ?wt ?wl ?wl ?es ?es Hres_type Hcg.
-    inv_cg_try_option Hres_type; subst.
-
-    destruct (Wasm_int.Int32.modulus <? length ρs_sum)%Z eqn:Hcmp; first inversion Hcg.
-    inv_cg_bind Hcg ?units ?wt ?wt ?wl ?wl ?es es_case1 Hret Hcg.
-    inv_cg_ret Hret; subst.
-    apply Z.ltb_ge in Hcmp.
-
-    inv_cg_bind Hcg ρs_atom ?wt ?wt ?wl ?wl ?es ?es Hιs Hcg.
-    inv_cg_try_option Hιs; subst.
-    inv_cg_bind Hcg val_localidxs wt_save ?wt wl_save ?wl es_save ?es Hsave Hcg.
-    repeat rewrite app_nil_r in Hsave.
-
-    (* Save tag *)
-    inv_cg_bind Hcg tag_localidx ?wt ?wt ?wl ?wl ?es ?es HsaveTag Hcg.
-    unfold save_stack1 in HsaveTag.
-    inv_cg_bind HsaveTag ?tl ?wt ?wt ?wl ?wl ?es ?es Halloc_tag HsaveTag.
-    apply wp_wlalloc in Halloc_tag as [Hlocal_tag_idx [-> [-> ->]]].
-    inv_cg_bind HsaveTag [] ?wt ?wt ?wl ?wl es_set_tag ?es HsetTag HretTagIdx.
-    inv_cg_emit HsetTag; subst.
-    inv_cg_ret HretTagIdx; subst.
-
-    clear_nils.
-    set (tag_idx := (fe_wlocal_offset fe + length (wl ++ wl_save))).
-    set (tag_localidx := Mk_localidx tag_idx).
-    replace (Mk_localidx (fe_wlocal_offset fe + length (wl ++ wl_save))) with tag_localidx in *; last done.
-
-    (* Put default result values on stack *)
-    inv_cg_bind Hcg [] ?wt ?wt ?wl ?wl es_create_defaults ?es Hcreate_defaults Hcg.
-    apply run_codegen_create_defaults in Hcreate_defaults as H.
-    destruct H as (_ & -> & -> & _).
-
-    (* Case blocks *)
-    cbv [map length seq zip Datatypes.uncurry] in Hcg.
-
-    clear_nils.
-
-    inv_cg_bind Hcg [] ?wt ?wt ?wl ?wl ?es es_case2 Hcase_es1 Hcase_es2.
-
-    (* Case es1 *)
-
-    inv_cg_bind Hcase_es1 ?pair ?wt ?wt ?wl ?wl ?es ?es Hcase_es1 Hcase_es1_block.
+    (* Case es_tag *)
+    inv_cg_bind Hcg_tag ?pair ?wt ?wt ?wl ?wl ?es ?es Hcase_es_tag Hcase_es_tag_block.
     destruct pair, u.
-    inv_cg_emit Hcase_es1_block; subst.
-    apply run_codegen_capture in Hcase_es1 as [Hcase_es1 ->].
+    inv_cg_emit Hcase_es_tag_block; subst.
+    apply run_codegen_capture in Hcase_es_tag as [Hcase_es_tag ->].
 
-    inv_cg_bind Hcase_es1 [] ?wt ?wt ?wl ?wl ?es ?es Hget_tag Hcase_es1.
+    inv_cg_bind Hcase_es_tag [] ?wt ?wt ?wl ?wl ?es ?es Hget_tag Hcase_es_tag.
     inv_cg_emit Hget_tag; subst.
 
-    inv_cg_bind Hcase_es1 [] ?wt ?wt ?wl ?wl ?es ?es Htag0 Hcase_es1.
+    inv_cg_bind Hcase_es_tag [] ?wt ?wt ?wl ?wl ?es ?es Htag0 Hcase_es_tag.
     inv_cg_emit Htag0; subst.
 
-    inv_cg_bind Hcase_es1 [] ?wt ?wt ?wl ?wl ?es ?es Hcompare_tag Hcase_es1.
+    inv_cg_bind Hcase_es_tag [] ?wt ?wt ?wl ?wl ?es ?es Hcompare_tag Hcase_es_tag.
     inv_cg_emit Hcompare_tag; subst.
 
-    inv_cg_bind Hcase_es1 [] ?wt ?wt ?wl ?wl ?es ?es Hbr_case Hcase_es1.
+    inv_cg_bind Hcase_es_tag [] ?wt ?wt ?wl ?wl ?es ?es Hbr_case Hcase_es_tag.
     inv_cg_emit Hbr_case; subst.
 
-    inv_cg_bind Hcase_es1 [] ?wt ?wt ?wl ?wl es_drop_1 ?es Hdrop_consts_1 Hcase_es1.
-    apply run_codegen_drop_consts in Hdrop_consts_1 as H.
+    inv_cg_bind Hcase_es_tag [] ?wt ?wt ?wl ?wl es_drop_tag ?es Hdrop_consts_tag Hcase_es_tag.
+    apply run_codegen_drop_consts in Hdrop_consts_tag as H.
     destruct H as (_ & -> & -> & _).
 
-    inv_cg_bind Hcase_es1 ρ_case1 ?wt ?wt ?wl ?wl ?es ?es Hlookup Hcase_es1.
+    inv_cg_bind Hcase_es_tag ρ_casetag ?wt ?wt ?wl ?wl ?es ?es Hlookup Hcase_es_tag.
     inv_cg_try_option Hlookup; subst.
 
-    inv_cg_bind Hcase_es1 case_1_sum_locals ?wt ?wt ?wl ?wl ?es ?es Hinject Hcase_es1.
+    inv_cg_bind Hcase_es_tag case_tag_sum_locals ?wt ?wt ?wl ?wl ?es ?es Hinject Hcase_es_tag.
     inv_cg_try_option Hinject; subst.
 
-    inv_cg_bind Hcase_es1 [] ?wt wt_case_1 ?wl wl_case_1 ?es es_case_1 Hget_locals_1 Hcase_es1.
-    inv_cg_bind Hget_locals_1 case_1_val_idxs ?wt wt_get_locals_1 ?wl wl_get_locals_1 ?es es_get_locals_1 Hnths_error Hget_locals_1.
+    inv_cg_bind Hcase_es_tag [] ?wt wt_case_tag ?wl wl_case_tag ?es es_case_tag Hget_locals_tag Hcase_es_tag.
+    inv_cg_bind Hget_locals_tag case_tag_val_idxs ?wt wt_get_locals_tag ?wl wl_get_locals_tag ?es es_get_locals_tag Hnths_error Hget_locals_tag.
     inv_cg_try_option Hnths_error; subst.
 
-    destruct (run_codegen_get_locals _ _ _ _ _ _ _ Hget_locals_1) as ([] & -> & ->).
-
-    clear_nils.
-
-    (* Case es2 *)
-
-    inv_cg_bind Hcase_es2 ?units ?wt ?wt ?wl ?wl ?es ?es Hcase_es2 Hmret.
-    inv_cg_ret Hmret; subst.
-
-    inv_cg_bind Hcase_es2 ?pair ?wt ?wt ?wl ?wl ?es ?es Hcase_es2 Hcase_es2_block.
-    destruct pair, u.
-    inv_cg_emit Hcase_es2_block; subst.
-    apply run_codegen_capture in Hcase_es2 as [Hcase_es2 ->].
-
-    inv_cg_bind Hcase_es2 [] ?wt ?wt ?wl ?wl ?es ?es Hget_tag Hcase_es2.
-    inv_cg_emit Hget_tag; subst.
-
-    inv_cg_bind Hcase_es2 [] ?wt ?wt ?wl ?wl ?es ?es Htag0 Hcase_es2.
-    inv_cg_emit Htag0; subst.
-
-    inv_cg_bind Hcase_es2 [] ?wt ?wt ?wl ?wl ?es ?es Hcompare_tag Hcase_es2.
-    inv_cg_emit Hcompare_tag; subst.
-
-    inv_cg_bind Hcase_es2 [] ?wt ?wt ?wl ?wl ?es ?es Hbr_case Hcase_es2.
-    inv_cg_emit Hbr_case; subst.
-
-    inv_cg_bind Hcase_es2 [] ?wt ?wt ?wl ?wl es_drop_2 ?es Hdrop_consts_2 Hcase_es2.
-    apply run_codegen_drop_consts in Hdrop_consts_2 as H.
-    destruct H as (_ & -> & -> & _).
-
-    inv_cg_bind Hcase_es2 ρ_case2 ?wt ?wt ?wl ?wl ?es ?es Hlookup Hcase_es2.
-    inv_cg_try_option Hlookup; subst.
-
-    inv_cg_bind Hcase_es2 case_2_sum_locals ?wt ?wt ?wl ?wl ?es ?es Hinject Hcase_es2.
-    inv_cg_try_option Hinject; subst.
-
-    inv_cg_bind Hcase_es2 [] ?wt wt_case_2 ?wl wl_case_2 ?es es_case_2 Hget_locals_2 Hcase_es2.
-    inv_cg_bind Hget_locals_2 case_2_val_idxs ?wt wt_get_locals_2 ?wl wl_get_locals_2 ?es es_get_locals_2 Hnths_error Hget_locals_2.
-    inv_cg_try_option Hnths_error; subst.
-
-    destruct (run_codegen_get_locals _ _ _ _ _ _ _ Hget_locals_2) as ([] & -> & ->).
+    destruct (run_codegen_get_locals _ _ _ _ _ _ _ Hget_locals_tag) as ([] & -> & ->).
 
     (* clean up *)
-    subst WT WL.
     clear_nils.
     simplify_eq.
 
-    (* Iris Proof *)
-    iIntros (? ? ? ? ? ? ? ?) "%Hsem %Hhas_values #Hinst #Hlabels #Hreturn Hrvs Hvs Hframe Hrt Hfr Hrun".
-    iDestruct (Hes1 _ _ (wt_case_2 ++ wtf) _ _ (wl_case_2 ++ wlf) _ Hcase_es1) as "Hsem_es1".
-    iDestruct (Hes2 _ _ wtf _ _ wlf _ Hcase_es2) as "Hsem_es2".
-
-    (* Our values are in the value interpretation for our specific SumT *)
-    (* This means that the values represent the tag and the payload. *)
-    iDestruct (values_interp_one_eq with "Hvs") as "Hvs".
-    iDestruct (value_interp_eq with "Hvs") as "Hvs".
-    unfold value_interp0, value_se_interp0.
-    iDestruct "Hvs" as "(%κ & %Hkind_sum & Hskind_as_type & Hsum_interp)".
-    (*unfold type_skind in Hkind_sum.*)
-    iDestruct "Hsum_interp" as (tag os' os_tag τ_tag ιs ιs_tag ixs  HSAtoms Htag_type_lookup Htag_type_arep Heval_rep_tail Hinject_sum_arep Hos'_ixs) "Hvalue_interp_os_i".
-    (*assert (os = I32A (Wasm_int.int_of_Z i32m i) :: os0) as ->; first by inversion HSAtoms.*)
-    simplify_eq.
-
-    apply lookup_lt_Some in Htag_type_lookup as Htag_size_bound.
-    assert (length τs = length ρs_sum) as Htyp_rep_len.
+    iApply (cwp_wand with "[-]").
     {
-      inversion Hok; subst.
-      unfold has_mono_rep_instr in H.
-      destruct H as [H _].
-      simpl in H.
-      rewrite Forall_singleton in H.
-      inversion H; subst.
-      inversion H1; subst.
-      apply has_kind_SumT_inv in H3 as (rf' & HF2).
-      by eapply Forall2_length.
+      (* iApply (compat_case_block_success with "[] [] [] [$] [$] [$] [$] [] [$] [$]"). *)
+      admit.
+
     }
-    assert (tag < Wasm_int.Int32.modulus)%Z as Htag_in_i32_bound.
-    { rewrite Htyp_rep_len in Htag_size_bound. eapply Z.lt_le_trans; last done. by apply Nat2Z.inj_lt. }
+    admit.
+
+Admitted.
+
+
+(*   Lemma compat_binary_case M F L L' wt wt' wtf wl wl' wlf es' ess es1 es2 τs τ1 τ2 τs' κ : *)
+(*     ess = [es1; es2] -> *)
+(*     τs = [τ1; τ2] -> *)
+(*     let fe := fe_of_context F in *)
+(*     let WT := wt ++ wt' ++ wtf in *)
+(*     let WL := wl ++ wl' ++ wlf in *)
+(*     let lmask := wlmask fe wl in *)
+(*     let F' := F <| fc_labels ::= cons (τs', L') |> in *)
+(*     let ψ := InstrT [SumT κ τs] τs' in *)
+(*     Forall2 *)
+(*       (fun τ es => *)
+(*          (forall wt wt' wtf wl wl' wlf es', *)
+(*             let fe' := fe_of_context F' in *)
+(*             let WT := wt ++ wt' ++ wtf in *)
+(*             let WL := wl ++ wl' ++ wlf in *)
+(*             let lmask := wlmask fe' wl in *)
+(*             run_codegen (compile_instrs mr fe' es) wt wl = inr ((), wt', wl', es') -> *)
+(*             ⊢ have_instr_type_sem rti sr mr M F' L WT WL lmask es' (InstrT [τ] τs') L')) *)
+(*       τs ess -> *)
+(*     has_instruction_type_ok F ψ L' -> *)
+(*     run_codegen (compile_instr mr fe (ICase ψ L' ess)) wt wl = inr ((), wt', wl', es') -> *)
+(*     ⊢ have_instr_type_sem rti sr mr M F L WT WL lmask es' ψ L'. *)
+(* Proof. *)
+(*     intros -> -> fe WT WL lmask F' Ψ Hforall Hok Hcg. *)
+(*     set (τs := [τ1; τ2]). *)
+(*     rewrite Forall2_cons_iff in Hforall. *)
+(*     destruct Hforall as [Hes1 H2]. *)
+(*     rewrite Forall2_cons_iff in H2. *)
+(*     destruct H2 as [Hes2 _]. *)
+(*     subst Ψ. *)
+(*     cbn [compile_instr] in Hcg. *)
+(*     destruct κ as [ ρ rf | ]; last inversion Hcg. *)
+(*     destruct ρ  as [ | ρs_sum | | ]; try done. *)
+(*     destruct τs' as [ | τ_res τs' ]; first done. *)
+(*     destruct τs'; last done. *)
+(**)
+(*     inv_cg_bind Hcg wl_ret ?wt ?wt ?wl ?wl ?es ?es Hres_type Hcg. *)
+(*     inv_cg_try_option Hres_type; subst. *)
+(**)
+(*     destruct (Wasm_int.Int32.modulus <? length ρs_sum)%Z eqn:Hcmp; first inversion Hcg. *)
+(*     inv_cg_bind Hcg ?units ?wt ?wt ?wl ?wl ?es es_case1 Hret Hcg. *)
+(*     inv_cg_ret Hret; subst. *)
+(*     apply Z.ltb_ge in Hcmp. *)
+(**)
+(*     inv_cg_bind Hcg ρs_atom ?wt ?wt ?wl ?wl ?es ?es Hιs Hcg. *)
+(*     inv_cg_try_option Hιs; subst. *)
+(*     inv_cg_bind Hcg val_localidxs wt_save ?wt wl_save ?wl es_save ?es Hsave Hcg. *)
+(*     repeat rewrite app_nil_r in Hsave. *)
+(**)
+(*     (* Save tag *) *)
+(*     inv_cg_bind Hcg tag_localidx ?wt ?wt ?wl ?wl ?es ?es HsaveTag Hcg. *)
+(*     unfold save_stack1 in HsaveTag. *)
+(*     inv_cg_bind HsaveTag ?tl ?wt ?wt ?wl ?wl ?es ?es Halloc_tag HsaveTag. *)
+(*     apply wp_wlalloc in Halloc_tag as [Hlocal_tag_idx [-> [-> ->]]]. *)
+(*     inv_cg_bind HsaveTag [] ?wt ?wt ?wl ?wl es_set_tag ?es HsetTag HretTagIdx. *)
+(*     inv_cg_emit HsetTag; subst. *)
+(*     inv_cg_ret HretTagIdx; subst. *)
+(**)
+(*     clear_nils. *)
+(*     set (tag_idx := (fe_wlocal_offset fe + length (wl ++ wl_save))). *)
+(*     set (tag_localidx := Mk_localidx tag_idx). *)
+(*     replace (Mk_localidx (fe_wlocal_offset fe + length (wl ++ wl_save))) with tag_localidx in *; last done. *)
+(**)
+(*     (* Put default result values on stack *) *)
+(*     inv_cg_bind Hcg [] ?wt ?wt ?wl ?wl es_create_defaults ?es Hcreate_defaults Hcg. *)
+(*     apply run_codegen_create_defaults in Hcreate_defaults as H. *)
+(*     destruct H as (_ & -> & -> & _). *)
+(**)
+(*     (* Case blocks *) *)
+(*     cbv [map length seq zip Datatypes.uncurry] in Hcg. *)
+(**)
+(*     clear_nils. *)
+(**)
+(*     inv_cg_bind Hcg [] ?wt ?wt ?wl ?wl ?es es_case2 Hcase_es1 Hcase_es2. *)
+(**)
+(*     (* Case es1 *) *)
+(**)
+(*     inv_cg_bind Hcase_es1 ?pair ?wt ?wt ?wl ?wl ?es ?es Hcase_es1 Hcase_es1_block. *)
+(*     destruct pair, u. *)
+(*     inv_cg_emit Hcase_es1_block; subst. *)
+(*     apply run_codegen_capture in Hcase_es1 as [Hcase_es1 ->]. *)
+(**)
+(*     inv_cg_bind Hcase_es1 [] ?wt ?wt ?wl ?wl ?es ?es Hget_tag Hcase_es1. *)
+(*     inv_cg_emit Hget_tag; subst. *)
+(**)
+(*     inv_cg_bind Hcase_es1 [] ?wt ?wt ?wl ?wl ?es ?es Htag0 Hcase_es1. *)
+(*     inv_cg_emit Htag0; subst. *)
+(**)
+(*     inv_cg_bind Hcase_es1 [] ?wt ?wt ?wl ?wl ?es ?es Hcompare_tag Hcase_es1. *)
+(*     inv_cg_emit Hcompare_tag; subst. *)
+(**)
+(*     inv_cg_bind Hcase_es1 [] ?wt ?wt ?wl ?wl ?es ?es Hbr_case Hcase_es1. *)
+(*     inv_cg_emit Hbr_case; subst. *)
+(**)
+(*     inv_cg_bind Hcase_es1 [] ?wt ?wt ?wl ?wl es_drop_1 ?es Hdrop_consts_1 Hcase_es1. *)
+(*     apply run_codegen_drop_consts in Hdrop_consts_1 as H. *)
+(*     destruct H as (_ & -> & -> & _). *)
+(**)
+(*     inv_cg_bind Hcase_es1 ρ_case1 ?wt ?wt ?wl ?wl ?es ?es Hlookup Hcase_es1. *)
+(*     inv_cg_try_option Hlookup; subst. *)
+(**)
+(*     inv_cg_bind Hcase_es1 case_1_sum_locals ?wt ?wt ?wl ?wl ?es ?es Hinject Hcase_es1. *)
+(*     inv_cg_try_option Hinject; subst. *)
+(**)
+(*     inv_cg_bind Hcase_es1 [] ?wt wt_case_1 ?wl wl_case_1 ?es es_case_1 Hget_locals_1 Hcase_es1. *)
+(*     inv_cg_bind Hget_locals_1 case_1_val_idxs ?wt wt_get_locals_1 ?wl wl_get_locals_1 ?es es_get_locals_1 Hnths_error Hget_locals_1. *)
+(*     inv_cg_try_option Hnths_error; subst. *)
+(**)
+(*     destruct (run_codegen_get_locals _ _ _ _ _ _ _ Hget_locals_1) as ([] & -> & ->). *)
+(**)
+(*     clear_nils. *)
+(**)
+(*     (* Case es2 *) *)
+(**)
+(*     inv_cg_bind Hcase_es2 ?units ?wt ?wt ?wl ?wl ?es ?es Hcase_es2 Hmret. *)
+(*     inv_cg_ret Hmret; subst. *)
+(**)
+(*     inv_cg_bind Hcase_es2 ?pair ?wt ?wt ?wl ?wl ?es ?es Hcase_es2 Hcase_es2_block. *)
+(*     destruct pair, u. *)
+(*     inv_cg_emit Hcase_es2_block; subst. *)
+(*     apply run_codegen_capture in Hcase_es2 as [Hcase_es2 ->]. *)
+(**)
+(*     inv_cg_bind Hcase_es2 [] ?wt ?wt ?wl ?wl ?es ?es Hget_tag Hcase_es2. *)
+(*     inv_cg_emit Hget_tag; subst. *)
+(**)
+(*     inv_cg_bind Hcase_es2 [] ?wt ?wt ?wl ?wl ?es ?es Htag0 Hcase_es2. *)
+(*     inv_cg_emit Htag0; subst. *)
+(**)
+(*     inv_cg_bind Hcase_es2 [] ?wt ?wt ?wl ?wl ?es ?es Hcompare_tag Hcase_es2. *)
+(*     inv_cg_emit Hcompare_tag; subst. *)
+(**)
+(*     inv_cg_bind Hcase_es2 [] ?wt ?wt ?wl ?wl ?es ?es Hbr_case Hcase_es2. *)
+(*     inv_cg_emit Hbr_case; subst. *)
+(**)
+(*     inv_cg_bind Hcase_es2 [] ?wt ?wt ?wl ?wl es_drop_2 ?es Hdrop_consts_2 Hcase_es2. *)
+(*     apply run_codegen_drop_consts in Hdrop_consts_2 as H. *)
+(*     destruct H as (_ & -> & -> & _). *)
+(**)
+(*     inv_cg_bind Hcase_es2 ρ_case2 ?wt ?wt ?wl ?wl ?es ?es Hlookup Hcase_es2. *)
+(*     inv_cg_try_option Hlookup; subst. *)
+(**)
+(*     inv_cg_bind Hcase_es2 case_2_sum_locals ?wt ?wt ?wl ?wl ?es ?es Hinject Hcase_es2. *)
+(*     inv_cg_try_option Hinject; subst. *)
+(**)
+(*     inv_cg_bind Hcase_es2 [] ?wt wt_case_2 ?wl wl_case_2 ?es es_case_2 Hget_locals_2 Hcase_es2. *)
+(*     inv_cg_bind Hget_locals_2 case_2_val_idxs ?wt wt_get_locals_2 ?wl wl_get_locals_2 ?es es_get_locals_2 Hnths_error Hget_locals_2. *)
+(*     inv_cg_try_option Hnths_error; subst. *)
+(**)
+(*     destruct (run_codegen_get_locals _ _ _ _ _ _ _ Hget_locals_2) as ([] & -> & ->). *)
+(**)
+(*     (* clean up *) *)
+(*     subst WT WL. *)
+(*     clear_nils. *)
+(*     simplify_eq. *)
+(**)
+(*     (* Iris Proof *) *)
+(*     iIntros (? ? ? ? ? ? ? ?) "%Hsem %Hhas_values #Hinst #Hlabels #Hreturn Hrvs Hvs Hframe Hrt Hfr Hrun". *)
+(*     iDestruct (Hes1 _ _ (wt_case_2 ++ wtf) _ _ (wl_case_2 ++ wlf) _ Hcase_es1) as "Hsem_es1". *)
+(*     iDestruct (Hes2 _ _ wtf _ _ wlf _ Hcase_es2) as "Hsem_es2". *)
+(**)
+(*     (* Our values are in the value interpretation for our specific SumT *) *)
+(*     (* This means that the values represent the tag and the payload. *) *)
+(*     iDestruct (values_interp_one_eq with "Hvs") as "Hvs". *)
+(*     iDestruct (value_interp_eq with "Hvs") as "Hvs". *)
+(*     unfold value_interp0, value_se_interp0. *)
+(*     iDestruct "Hvs" as "(%κ & %Hkind_sum & Hskind_as_type & Hsum_interp)". *)
+(*     (*unfold type_skind in Hkind_sum.*) *)
+(*     iDestruct "Hsum_interp" as (tag os' os_tag τ_tag ιs ιs_tag ixs  HSAtoms Htag_type_lookup Htag_type_arep Heval_rep_tail Hinject_sum_arep Hos'_ixs) "Hvalue_interp_os_i". *)
+(*     (*assert (os = I32A (Wasm_int.int_of_Z i32m i) :: os0) as ->; first by inversion HSAtoms.*) *)
+(*     simplify_eq. *)
+(**)
+(*     apply lookup_lt_Some in Htag_type_lookup as Htag_size_bound. *)
+(*     assert (length τs = length ρs_sum) as Htyp_rep_len. *)
+(*     { *)
+(*       inversion Hok; subst. *)
+(*       unfold has_mono_rep_instr in H. *)
+(*       destruct H as [H _]. *)
+(*       simpl in H. *)
+(*       rewrite Forall_singleton in H. *)
+(*       inversion H; subst. *)
+(*       inversion H1; subst. *)
+(*       apply has_kind_SumT_inv in H3 as (rf' & HF2). *)
+(*       by eapply Forall2_length. *)
+(*     } *)
+(*     assert (tag < Wasm_int.Int32.modulus)%Z as Htag_in_i32_bound. *)
+(*     { rewrite Htyp_rep_len in Htag_size_bound. eapply Z.lt_le_trans; last done. by apply Nat2Z.inj_lt. } *)
+(**)
+(*     (* TODO: we should also know that tag < length (ρs_sum). This will follow easily from the above and Htag_type_lookup *) *)
+(**)
+(*     iDestruct (big_sepL2_length with "Hrvs") as "%Hlen". *)
+(*     destruct vs as [|v_tag vs_payload]; first inversion Hlen. *)
+(*     clear Hlen. *)
+(*     iDestruct (atoms_interp_cons with "Hrvs") as "[-> Hatoms_interp_payload]". *)
+(**)
+(*     iPoseProof (frame_interp_wl_interp with "Hframe") as "%Hwl"; first done. *)
+(*     rewrite list_extra.cons_app in Hhas_values. *)
+(*     apply has_values_app_inv in Hhas_values as (e_tag & es_payload & -> & Hhv_tag & Hhvs_payload). *)
+(**)
+(*     (* save payload *) *)
+(*     rewrite (app_assoc (e_tag ++ _)). *)
+(*     iApply (cwp_seq with "[Hfr Hrun]"). *)
+(*     { *)
+(*       rewrite <- (app_assoc e_tag). *)
+(*       instantiate (1 := λ fr' vs, ( *)
+(*         ∃ val_idxs, *)
+(*         ⌜vs = [VAL_int32 (Wasm_int.Int32.repr tag)]⌝ ∗ *)
+(*         ⌜frame_rel (λ i, i ∉ val_idxs) fr fr'⌝ ∗ *)
+(*         ⌜Forall2 (fun i v => f_locs fr' !! localimm i = Some v) val_localidxs vs_payload⌝ ∗ *)
+(*         ⌜val_idxs = seq (fe_wlocal_offset fe + length wl) (length wl_save)⌝ ∗ *)
+(*         ⌜val_localidxs = map prelude.W.Mk_localidx val_idxs⌝ *)
+(*         )%I). *)
+(*       iApply cwp_val_app; first done. *)
+(*       eapply cwp_save_stack_w in Hsave; eauto. *)
+(*       + destruct Hsave as (-> & -> & -> & Hsave). *)
+(*         iApply (Hsave with "[$] [$]"). *)
+(*         iIntros (f' [Hfsame Hfchanged]). *)
+(*         unfold fvs_combine. *)
+(*         auto. *)
+(*       + admit. (* easy pure conseqeunce of value_interp and *)
+(*       rep_values_interp, should be proved above the first wp_seq *)
+(*       rule *) *)
+(*     } *)
+(*     iIntros (fr_saved w) "(%val_idxs & -> & %Hfrel_fr_saved & %Hsaved & %Hval_idxs_seq & %Hval_localidxs) Hfr Hrun". *)
+(*     iAssert *)
+(*       (frame_interp rti sr se L (wl ++ wl_save ++ [prelude.W.T_i32] ++ wl_case_1 ++ wl_case_2 ++ wlf) fr_saved) *)
+(*       with "[Hframe]" as "Hframe_saved". *)
+(*     { admit. } (* TODO: Not really sure how to prove this. Definitely need helper lemma *) *)
+(**)
+(*     edestruct (util.nths_error_exists val_localidxs case_1_val_idxs vs_payload case_1_sum_locals (Forall2_length _ _ _ Hsaved)) as [case_1_vs_payload Hnerr_payload_c1]; try done. *)
+(**)
+(*     edestruct (util.nths_error_exists val_localidxs case_2_val_idxs vs_payload case_2_sum_locals (Forall2_length _ _ _ Hsaved)) as [case_2_vs_payload Hnerr_payload_c2]; try done. *)
+(**)
+(*     iDestruct (frame_interp_wl_interp with "Hframe_saved") as "%Hwl_saved"; first done. *)
+(*     pose proof (interp_wl_length _ _ _ Hwl_saved) as Hfr_saved_locs_len. *)
+(**)
+(*     assert (tag_idx < length (f_locs fr_saved)) as Htag_in_fr_saved. *)
+(*     { *)
+(*       subst tag_idx. *)
+(*       simpl. *)
+(*       eapply Nat.lt_le_trans; last done. *)
+(*       - rewrite app_assoc. *)
+(*         subst fe. *)
+(*         instantiate (1 := F). *)
+(*         repeat rewrite length_app. *)
+(*         lias. *)
+(*     } *)
+(**)
+(*     (* Store tag *) *)
+(*     rewrite (app_assoc (map _ _)). *)
+(*     iApply (cwp_seq with "[Hfr Hrun]"). *)
+(*     { *)
+(*       instantiate (1 := λ fr' vs, ( *)
+(*         ⌜vs = []⌝ ∗ *)
+(*         ⌜frame_rel (λ j, j ≠ tag_idx) fr_saved fr'⌝ ∗ *)
+(*         ⌜f_locs fr' !! tag_idx = Some (VAL_int32 (Wasm_int.Int32.repr tag))⌝ *)
+(*         )%I). *)
+(*       iApply (cwp_local_set with "[] [$] [$]"); first done. *)
+(*       iSplit; first done. *)
+(*       iSplit. *)
+(*       - iPureIntro. *)
+(*         split; last done. *)
+(*         intros j Hneq. *)
+(*         simpl. *)
+(*         rewrite list_lookup_insert_ne; [reflexivity | lia]. *)
+(*       - iSimpl. *)
+(*         iPureIntro. *)
+(*         rewrite list_lookup_insert_eq; try done. *)
+(*     } *)
+(*     iIntros (fr_saved_and_tag w) "(-> & %Hfrel_fr_saved_and_tag & %Hsaved_and_tag) Hfr Hrun". *)
+(*     clear_nils. *)
+(**)
+(*     (* relate starting frame fr and fr_saved_and_tag *) *)
+(*     pose proof (frame_rel_mask_trans_combine _ _ _ _ _ Hfrel_fr_saved Hfrel_fr_saved_and_tag) as Hfrel_fr_and_fr_saved_and_tag. *)
+(*     simpl in Hfrel_fr_and_fr_saved_and_tag. *)
+(**)
+(*     assert (frame_rel lmask fr fr_saved_and_tag) as Hfrel_lmask_saved_and_tag. *)
+(*     { *)
+(*       eapply frame_rel_mask_mono; [| exact Hfrel_fr_and_fr_saved_and_tag]. *)
+(*       intros i [Hi_lo Hi_hi]. *)
+(*       split. *)
+(*       + rewrite Hval_idxs_seq. *)
+(*         intro Hin. apply elem_of_seq in Hin. lia. *)
+(*       + unfold tag_idx. rewrite length_app. lia. *)
+(*     } *)
+(*     pose proof Hfrel_fr_and_fr_saved_and_tag as [_ ->]. *)
+(*     iDestruct (labels_interp_mono _ _ _ _ fr_saved_and_tag _ _ _ _ with "Hlabels") as "Hlabels'"; first done. *)
+(*     { *)
+(*       instantiate (1 := (wlmask (fe_of_context F') (wl ++ wl_save ++ [prelude.W.T_i32]))). *)
+(*       intros i [Hi_lo Hi_hi]. *)
+(*       simpl. *)
+(*       split. *)
+(*       + exact Hi_lo. *)
+(*       + rewrite -fe_of_context_labels. *)
+(*         rewrite !length_app. simpl. *)
+(*         subst fe. *)
+(*         lia. *)
+(*     } *)
+(**)
+(*     assert (Forall2 (λ (i : prelude.W.localidx) (v : value), f_locs fr_saved_and_tag !! localimm i = Some v) *)
+(*       val_localidxs vs_payload) as Hfr_saved_and_tag_payload. *)
+(*     { *)
+(*       eapply forall2_lookup_same. *)
+(*       3: done. *)
+(*       - intros. instantiate (1 := tag_idx) in H. *)
+(*         destruct Hfrel_fr_saved_and_tag as [-> _]; done. *)
+(*       - subst val_idxs val_localidxs tag_idx. *)
+(*         rewrite length_app Nat.add_assoc. *)
+(*         apply map_seq_forall_localidx_neq. *)
+(*     } *)
+(**)
+(*     iAssert *)
+(*       (frame_interp rti sr se L (wl ++ wl_save ++ [prelude.W.T_i32] ++ wl_case_1 ++ wl_case_2 ++ wlf) fr_saved_and_tag) *)
+(*       with "[Hframe_saved]" as "Hframe_saved_and_tag". *)
+(*     { admit. } (* TODO: Not really sure how to prove this. Definitely need helper lemma *) *)
+(**)
+(*     (* Create defaults *) *)
+(*     iApply (cwp_seq with "[Hfr Hrun]"). *)
+(*     { *)
+(*       eapply cwp_create_defaults in Hcreate_defaults as (_ & _ & _ & Hcreate_defaults). *)
+(*       iDestruct (Hcreate_defaults with "[$] [$] []") as "Hcreate_defaults". *)
+(*       { *)
+(*         by instantiate (1 := λ f vs, (⌜f = fr_saved_and_tag⌝ ∗ ⌜vs = (map default_of_value_type wl_ret)⌝)%I). *)
+(*       } *)
+(*       iApply "Hcreate_defaults". *)
+(*     } *)
+(*     iIntros (??) "[-> ->] Hfr Hrun". *)
+(**)
+(*     (* Case analysis: Is tag 0 or 1? *) *)
+(**)
+(*     apply lookup_lt_Some in Htag_type_lookup as Hi. *)
+(*     destruct tag as [| [|]]; last done. *)
+(**)
+(*     - (* Case: tag = 0 *) *)
+(*       (* -------- Case 1 -------- *) *)
+(*       rewrite (app_assoc (to_consts _)). *)
+(*       iApply (cwp_seq with "[-]"). *)
+(*       { *)
+(*         iApply (compat_case_block_success with "[] [$] [$] [$] [$] [$] [$] [$] [$] [$]"). *)
+(*         2: instantiate (1 := []). *)
+(*         all: clear_nils. *)
+(*         1, 2, 3, 4, 5, 6, 8, 9, 11, 13, 14: done. *)
+(*         4: iApply "Hsem_es1". *)
+(*         1: done. *)
+(*         1: by rewrite length_map. *)
+(*         by subst val_idxs. *)
+(*       } *)
+(*       iIntros (f_es_case_1 vs) "(_ & %Hlen_vs & %Hfrel_new & Hframe & %os & %θ' & Hos & Hvs & Hrt) Hfr Hrun". *)
+(**)
+(*       (* -------- Case 2 -------- *) *)
+(*       iApply (cwp_wand with "[Hfr Hrun]"). *)
+(*       { *)
+(*         iApply (compat_case_block_fail with "[$] [$]"). *)
+(*         3: by instantiate (1 := 0). *)
+(*         2, 3, 4, 5: done. *)
+(*         rewrite -Hsaved_and_tag. *)
+(*         destruct Hfrel_new as [Hmask _]. *)
+(*         symmetry. *)
+(*         apply Hmask. *)
+(*         subst tag_idx fe. *)
+(*         unfold wlmask. *)
+(*         repeat rewrite length_app. *)
+(*         rewrite -fe_of_context_labels. *)
+(*         lias. *)
+(*       } *)
+(*       (* iIntros (??) "(-> & ->) Hfr Hrun". *) *)
+(*       (* TODO: we would probably want fr and run resource back from the block_fail lemma *) *)
+(*       iIntros (??) "(-> & ->)". *)
+(*       iFrame. *)
+(*       iPureIntro. *)
+(*       rewrite -fe_of_context_labels in Hfrel_new. *)
+(*       unfold lmask. *)
+(*       eapply frame_rel_trans. *)
+(*       + eapply frame_rel_mask_mono; [| exact Hfrel_lmask_saved_and_tag]. *)
+(*         intros i [Hi_lo Hi_hi]. unfold lmask, wlmask. split; exact Hi_lo || exact Hi_hi. *)
+(*       + eapply frame_rel_wlmask_mono; [| exact Hfrel_new]. *)
+(*         rewrite length_app. lia. *)
+(**)
+(*     - (* Case: tag = 1 *) *)
+(*       (* -------- Case 1 -------- *) *)
+(*       rewrite (app_assoc (to_consts _)). *)
+(*       iApply (cwp_seq with "[Hfr Hrun]"). *)
+(*       { *)
+(*         iApply (compat_case_block_fail with "[$] [$]"). *)
+(*         3: by instantiate (1 := 1). *)
+(*         1, 2, 3, 4: done. *)
+(*         by rewrite length_map. *)
+(*       } *)
+(*       iIntros (??) "(-> & ->) Hfr Hrun". *)
+(**)
+(*       iDestruct (labels_interp_mono _ _ _ _ fr_saved_and_tag _ _ _ _ with "Hlabels") as "Hlabels'''"; first done. *)
+(*       { *)
+(*         instantiate (1 := (wlmask (fe_of_context F') (wl ++ wl_save ++ [prelude.W.T_i32] ++ wl_case_1))). *)
+(*         intros i [Hi_lo Hi_hi]. *)
+(*         simpl. *)
+(*         split. *)
+(*         + exact Hi_lo. *)
+(*         + rewrite -fe_of_context_labels. *)
+(*           rewrite !length_app. simpl. *)
+(*           subst fe. *)
+(*           lia. *)
+(*       } *)
+(**)
+(*       (* -------- Case 2 -------- *) *)
+(*       iApply (cwp_wand with "[-]"). *)
+(*       { *)
+(*         iApply (compat_case_block_success with "[] [$] [$] [$] [$] [$] [$] [$] [$] [$]"). *)
+(*         1, 2, 3, 4, 5, 6, 8, 9, 11, 13, 14, 15: done. *)
+(*         1: done. *)
+(*         1: by rewrite length_map. *)
+(*         by subst val_idxs. *)
+(*       } *)
+(*       iIntros (f_es_case_2 vs) "(_ & %Hlen_vs & %Hfrel_new & Hframe & %os & %θ' & Hos & Hvs & Hrt)". *)
+(*       iFrame. *)
+(*       iPureIntro. *)
+(*       rewrite -fe_of_context_labels in Hfrel_new. *)
+(*       unfold lmask. *)
+(*       eapply frame_rel_trans. *)
+(*       + eapply frame_rel_mask_mono; [| exact Hfrel_lmask_saved_and_tag]. *)
+(*         intros i [Hi_lo Hi_hi]. unfold lmask, wlmask. split; exact Hi_lo || exact Hi_hi. *)
+(*       + eapply frame_rel_wlmask_mono; [| exact Hfrel_new]. *)
+(*         rewrite length_app. lia. *)
+(*   Admitted. *)
+(**)
+(**)
+(*   Lemma compat_ternary_case M F L L' wt wt' wtf wl wl' wlf es' ess es1 es2 es3 τs τ1 τ2 τ3 τs' κ : *)
+(*     ess = [es1; es2; es3] -> *)
+(*     τs = [τ1; τ2; τ3] -> *)
+(*     let fe := fe_of_context F in *)
+(*     let WT := wt ++ wt' ++ wtf in *)
+(*     let WL := wl ++ wl' ++ wlf in *)
+(*     let lmask := wlmask fe wl in *)
+(*     let F' := F <| fc_labels ::= cons (τs', L') |> in *)
+(*     let ψ := InstrT [SumT κ τs] τs' in *)
+(*     Forall2 *)
+(*       (fun τ es => *)
+(*          (forall wt wt' wtf wl wl' wlf es', *)
+(*             let fe' := fe_of_context F' in *)
+(*             let WT := wt ++ wt' ++ wtf in *)
+(*             let WL := wl ++ wl' ++ wlf in *)
+(*             let lmask := wlmask fe' wl in *)
+(*             run_codegen (compile_instrs mr fe' es) wt wl = inr ((), wt', wl', es') -> *)
+(*             ⊢ have_instr_type_sem rti sr mr M F' L WT WL lmask es' (InstrT [τ] τs') L')) *)
+(*       τs ess -> *)
+(*     has_instruction_type_ok F ψ L' -> *)
+(*     run_codegen (compile_instr mr fe (ICase ψ L' ess)) wt wl = inr ((), wt', wl', es') -> *)
+(*     ⊢ have_instr_type_sem rti sr mr M F L WT WL lmask es' ψ L'. *)
+(* Proof. *)
+(*     intros -> -> fe WT WL lmask F' Ψ Hforall Hok Hcg. *)
+(*     set (τs := [τ1; τ2; τ3]). *)
+(*     rewrite Forall2_cons_iff in Hforall. *)
+(*     destruct Hforall as [Hes1 H2]. *)
+(*     rewrite Forall2_cons_iff in H2. *)
+(*     destruct H2 as [Hes2 H3]. *)
+(*     rewrite Forall2_cons_iff in H3. *)
+(*     destruct H3 as [Hes3 _]. *)
+(*     subst Ψ. *)
+(*     cbn [compile_instr] in Hcg. *)
+(*     destruct κ as [ ρ rf | ]; last inversion Hcg. *)
+(*     destruct ρ  as [ | ρs_sum | | ]; try done. *)
+(*     destruct τs' as [ | τ_res τs' ]; first done. *)
+(*     destruct τs'; last done. *)
+(**)
+(*     inv_cg_bind Hcg wl_ret ?wt ?wt ?wl ?wl ?es ?es Hres_type Hcg. *)
+(*     inv_cg_try_option Hres_type; subst. *)
+(**)
+(*     destruct (Wasm_int.Int32.modulus <? length ρs_sum)%Z eqn:Hcmp; first inversion Hcg. *)
+(*     inv_cg_bind Hcg ?units ?wt ?wt ?wl ?wl ?es es_case1 Hret Hcg. *)
+(*     inv_cg_ret Hret; subst. *)
+(*     apply Z.ltb_ge in Hcmp. *)
+(**)
+(*     inv_cg_bind Hcg ρs_atom ?wt ?wt ?wl ?wl ?es ?es Hιs Hcg. *)
+(*     inv_cg_try_option Hιs; subst. *)
+(*     inv_cg_bind Hcg val_localidxs wt_save ?wt wl_save ?wl es_save ?es Hsave Hcg. *)
+(*     repeat rewrite app_nil_r in Hsave. *)
+(**)
+(*     (* Save tag *) *)
+(*     inv_cg_bind Hcg tag_localidx ?wt ?wt ?wl ?wl ?es ?es HsaveTag Hcg. *)
+(*     unfold save_stack1 in HsaveTag. *)
+(*     inv_cg_bind HsaveTag ?tl ?wt ?wt ?wl ?wl ?es ?es Halloc_tag HsaveTag. *)
+(*     apply wp_wlalloc in Halloc_tag as [Hlocal_tag_idx [-> [-> ->]]]. *)
+(*     inv_cg_bind HsaveTag [] ?wt ?wt ?wl ?wl es_set_tag ?es HsetTag HretTagIdx. *)
+(*     inv_cg_emit HsetTag; subst. *)
+(*     inv_cg_ret HretTagIdx; subst. *)
+(**)
+(*     clear_nils. *)
+(*     set (tag_idx := (fe_wlocal_offset fe + length (wl ++ wl_save))). *)
+(*     set (tag_localidx := Mk_localidx tag_idx). *)
+(*     replace (Mk_localidx (fe_wlocal_offset fe + length (wl ++ wl_save))) with tag_localidx in *; last done. *)
+(**)
+(*     (* Put default result values on stack *) *)
+(*     inv_cg_bind Hcg [] ?wt ?wt ?wl ?wl es_create_defaults ?es Hcreate_defaults Hcg. *)
+(*     apply run_codegen_create_defaults in Hcreate_defaults as H. *)
+(*     destruct H as (_ & -> & -> & _). *)
+(**)
+(*     (* Case blocks *) *)
+(*     cbv [map length seq zip Datatypes.uncurry] in Hcg. *)
+(**)
+(*     clear_nils. *)
+(**)
+(*     inv_cg_bind Hcg [] ?wt ?wt ?wl ?wl ?es es_case2 Hcase_es1 Hcases. *)
+(*     inv_cg_bind Hcases [] ?wt ?wt ?wl ?wl ?es ?es Hcase_es2 Hcase_es3. *)
+(**)
+(*     (* Case es1 *) *)
+(**)
+(*     inv_cg_bind Hcase_es1 ?pair ?wt ?wt ?wl ?wl ?es ?es Hcase_es1 Hcase_es1_block. *)
+(*     destruct pair, u. *)
+(*     inv_cg_emit Hcase_es1_block; subst. *)
+(*     apply run_codegen_capture in Hcase_es1 as [Hcase_es1 ->]. *)
+(**)
+(*     inv_cg_bind Hcase_es1 [] ?wt ?wt ?wl ?wl ?es ?es Hget_tag Hcase_es1. *)
+(*     inv_cg_emit Hget_tag; subst. *)
+(**)
+(*     inv_cg_bind Hcase_es1 [] ?wt ?wt ?wl ?wl ?es ?es Htag0 Hcase_es1. *)
+(*     inv_cg_emit Htag0; subst. *)
+(**)
+(*     inv_cg_bind Hcase_es1 [] ?wt ?wt ?wl ?wl ?es ?es Hcompare_tag Hcase_es1. *)
+(*     inv_cg_emit Hcompare_tag; subst. *)
+(**)
+(*     inv_cg_bind Hcase_es1 [] ?wt ?wt ?wl ?wl ?es ?es Hbr_case Hcase_es1. *)
+(*     inv_cg_emit Hbr_case; subst. *)
+(**)
+(*     inv_cg_bind Hcase_es1 [] ?wt ?wt ?wl ?wl es_drop_1 ?es Hdrop_consts_1 Hcase_es1. *)
+(*     apply run_codegen_drop_consts in Hdrop_consts_1 as H. *)
+(*     destruct H as (_ & -> & -> & _). *)
+(**)
+(*     inv_cg_bind Hcase_es1 ρ_case1 ?wt ?wt ?wl ?wl ?es ?es Hlookup Hcase_es1. *)
+(*     inv_cg_try_option Hlookup; subst. *)
+(**)
+(*     inv_cg_bind Hcase_es1 case_1_sum_locals ?wt ?wt ?wl ?wl ?es ?es Hinject Hcase_es1. *)
+(*     inv_cg_try_option Hinject; subst. *)
+(**)
+(*     inv_cg_bind Hcase_es1 [] ?wt wt_case_1 ?wl wl_case_1 ?es es_case_1 Hget_locals_1 Hcase_es1. *)
+(*     inv_cg_bind Hget_locals_1 case_1_val_idxs ?wt wt_get_locals_1 ?wl wl_get_locals_1 ?es es_get_locals_1 Hnths_error Hget_locals_1. *)
+(*     inv_cg_try_option Hnths_error; subst. *)
+(**)
+(*     destruct (run_codegen_get_locals _ _ _ _ _ _ _ Hget_locals_1) as ([] & -> & ->). *)
+(**)
+(*     clear_nils. *)
+(**)
+(*     (* Case es2 *) *)
+(**)
+(*     inv_cg_bind Hcase_es2 ?pair ?wt ?wt ?wl ?wl ?es ?es Hcase_es2 Hcase_es2_block. *)
+(*     destruct pair, u. *)
+(*     inv_cg_emit Hcase_es2_block; subst. *)
+(*     apply run_codegen_capture in Hcase_es2 as [Hcase_es2 ->]. *)
+(**)
+(*     inv_cg_bind Hcase_es2 [] ?wt ?wt ?wl ?wl ?es ?es Hget_tag Hcase_es2. *)
+(*     inv_cg_emit Hget_tag; subst. *)
+(**)
+(*     inv_cg_bind Hcase_es2 [] ?wt ?wt ?wl ?wl ?es ?es Htag0 Hcase_es2. *)
+(*     inv_cg_emit Htag0; subst. *)
+(**)
+(*     inv_cg_bind Hcase_es2 [] ?wt ?wt ?wl ?wl ?es ?es Hcompare_tag Hcase_es2. *)
+(*     inv_cg_emit Hcompare_tag; subst. *)
+(**)
+(*     inv_cg_bind Hcase_es2 [] ?wt ?wt ?wl ?wl ?es ?es Hbr_case Hcase_es2. *)
+(*     inv_cg_emit Hbr_case; subst. *)
+(**)
+(*     inv_cg_bind Hcase_es2 [] ?wt ?wt ?wl ?wl es_drop_2 ?es Hdrop_consts_2 Hcase_es2. *)
+(*     apply run_codegen_drop_consts in Hdrop_consts_2 as H. *)
+(*     destruct H as (_ & -> & -> & _). *)
+(**)
+(*     inv_cg_bind Hcase_es2 ρ_case2 ?wt ?wt ?wl ?wl ?es ?es Hlookup Hcase_es2. *)
+(*     inv_cg_try_option Hlookup; subst. *)
+(**)
+(*     inv_cg_bind Hcase_es2 case_2_sum_locals ?wt ?wt ?wl ?wl ?es ?es Hinject Hcase_es2. *)
+(*     inv_cg_try_option Hinject; subst. *)
+(**)
+(*     inv_cg_bind Hcase_es2 [] ?wt wt_case_2 ?wl wl_case_2 ?es es_case_2 Hget_locals_2 Hcase_es2. *)
+(*     inv_cg_bind Hget_locals_2 case_2_val_idxs ?wt wt_get_locals_2 ?wl wl_get_locals_2 ?es es_get_locals_2 Hnths_error Hget_locals_2. *)
+(*     inv_cg_try_option Hnths_error; subst. *)
+(**)
+(*     destruct (run_codegen_get_locals _ _ _ _ _ _ _ Hget_locals_2) as ([] & -> & ->). *)
+(**)
+(**)
+(*     (* Case es3 *) *)
+(*     inv_cg_bind Hcase_es3 ?units ?wt ?wt ?wl ?wl ?es ?es Hcase_es3 Hmret. *)
+(*     inv_cg_ret Hmret; subst. *)
+(**)
+(*     inv_cg_bind Hcase_es3 ?pair ?wt ?wt ?wl ?wl ?es ?es Hcase_es3 Hcase_es3_block. *)
+(*     destruct pair, u. *)
+(*     inv_cg_emit Hcase_es3_block; subst. *)
+(*     apply run_codegen_capture in Hcase_es3 as [Hcase_es3 ->]. *)
+(**)
+(*     inv_cg_bind Hcase_es3 [] ?wt ?wt ?wl ?wl ?es ?es Hget_tag Hcase_es3. *)
+(*     inv_cg_emit Hget_tag; subst. *)
+(**)
+(*     inv_cg_bind Hcase_es3 [] ?wt ?wt ?wl ?wl ?es ?es Htag0 Hcase_es3. *)
+(*     inv_cg_emit Htag0; subst. *)
+(**)
+(*     inv_cg_bind Hcase_es3 [] ?wt ?wt ?wl ?wl ?es ?es Hcompare_tag Hcase_es3. *)
+(*     inv_cg_emit Hcompare_tag; subst. *)
+(**)
+(*     inv_cg_bind Hcase_es3 [] ?wt ?wt ?wl ?wl ?es ?es Hbr_case Hcase_es3. *)
+(*     inv_cg_emit Hbr_case; subst. *)
+(**)
+(*     inv_cg_bind Hcase_es3 [] ?wt ?wt ?wl ?wl es_drop_3 ?es Hdrop_consts_3 Hcase_es3. *)
+(*     apply run_codegen_drop_consts in Hdrop_consts_3 as H. *)
+(*     destruct H as (_ & -> & -> & _). *)
+(**)
+(*     inv_cg_bind Hcase_es3 ρ_case3 ?wt ?wt ?wl ?wl ?es ?es Hlookup Hcase_es3. *)
+(*     inv_cg_try_option Hlookup; subst. *)
+(**)
+(*     inv_cg_bind Hcase_es3 case_3_sum_locals ?wt ?wt ?wl ?wl ?es ?es Hinject Hcase_es3. *)
+(*     inv_cg_try_option Hinject; subst. *)
+(**)
+(*     inv_cg_bind Hcase_es3 [] ?wt wt_case_3 ?wl wl_case_3 ?es es_case_3 Hget_locals_3 Hcase_es3. *)
+(*     inv_cg_bind Hget_locals_3 case_3_val_idxs ?wt wt_get_locals_3 ?wl wl_get_locals_3 ?es es_get_locals_3 Hnths_error Hget_locals_3. *)
+(*     inv_cg_try_option Hnths_error; subst. *)
+(**)
+(*     destruct (run_codegen_get_locals _ _ _ _ _ _ _ Hget_locals_3) as ([] & -> & ->). *)
+(**)
+(**)
+(*     (* clean up *) *)
+(*     subst WT WL. *)
+(*     clear_nils. *)
+(*     simplify_eq. *)
+(**)
+(*     (* Iris Proof *) *)
+(*     iIntros (? ? ? ? ? ? ? ?) "%Hsem %Hhas_values #Hinst #Hlabels #Hreturn Hrvs Hvs Hframe Hrt Hfr Hrun". *)
+(*     iDestruct (Hes1 _ _ (wt_case_2 ++ wt_case_3 ++ wtf) _ _ (wl_case_2 ++ wl_case_3 ++ wlf) _ Hcase_es1) as "Hsem_es1". *)
+(*     iDestruct (Hes2 _ _ (wt_case_3 ++ wtf) _ _ (wl_case_3 ++ wlf) _ Hcase_es2) as "Hsem_es2". *)
+(*     iDestruct (Hes3 _ _ (wtf) _ _ (wlf) _ Hcase_es3) as "Hsem_es3". *)
+(**)
+(*     (* Our values are in the value interpretation for our specific SumT *) *)
+(*     (* This means that the values represent the tag and the payload. *) *)
+(*     iDestruct (values_interp_one_eq with "Hvs") as "Hvs". *)
+(*     iDestruct (value_interp_eq with "Hvs") as "Hvs". *)
+(*     unfold value_interp0, value_se_interp0. *)
+(*     iDestruct "Hvs" as "(%κ & %Hkind_sum & Hskind_as_type & Hsum_interp)". *)
+(*     (*unfold type_skind in Hkind_sum.*) *)
+(*     iDestruct "Hsum_interp" as (tag os' os_tag τ_tag ιs ιs_tag ixs  HSAtoms Htag_type_lookup Htag_type_arep Heval_rep_tail Hinject_sum_arep Hos'_ixs) "Hvalue_interp_os_i". *)
+(*     (*assert (os = I32A (Wasm_int.int_of_Z i32m i) :: os0) as ->; first by inversion HSAtoms.*) *)
+(*     simplify_eq. *)
+(**)
+(*     apply lookup_lt_Some in Htag_type_lookup as Htag_size_bound. *)
+(*     assert (length τs = length ρs_sum) as Htyp_rep_len. *)
+(*     { *)
+(*       inversion Hok; subst. *)
+(*       unfold has_mono_rep_instr in H. *)
+(*       destruct H as [H _]. *)
+(*       simpl in H. *)
+(*       rewrite Forall_singleton in H. *)
+(*       inversion H; subst. *)
+(*       inversion H1; subst. *)
+(*       apply has_kind_SumT_inv in H3 as (rf' & HF2). *)
+(*       by eapply Forall2_length. *)
+(*     } *)
+(*     assert (tag < Wasm_int.Int32.modulus)%Z as Htag_in_i32_bound. *)
+(*     { rewrite Htyp_rep_len in Htag_size_bound. eapply Z.lt_le_trans; last done. by apply Nat2Z.inj_lt. } *)
+(**)
+(*     iDestruct (big_sepL2_length with "Hrvs") as "%Hlen". *)
+(*     destruct vs as [|v_tag vs_payload]; first inversion Hlen. *)
+(*     clear Hlen. *)
+(*     iDestruct (atoms_interp_cons with "Hrvs") as "[-> Hatoms_interp_payload]". *)
+(**)
+(*     iPoseProof (frame_interp_wl_interp with "Hframe") as "%Hwl"; first done. *)
+(*     rewrite list_extra.cons_app in Hhas_values. *)
+(*     apply has_values_app_inv in Hhas_values as (e_tag & es_payload & -> & Hhv_tag & Hhvs_payload). *)
+(**)
+(*     (* save payload *) *)
+(*     rewrite (app_assoc (e_tag ++ _)). *)
+(*     iApply (cwp_seq with "[Hfr Hrun]"). *)
+(*     { *)
+(*       rewrite <- (app_assoc e_tag). *)
+(*       instantiate (1 := λ fr' vs, ( *)
+(*         ∃ val_idxs, *)
+(*         ⌜vs = [VAL_int32 (Wasm_int.Int32.repr tag)]⌝ ∗ *)
+(*         ⌜frame_rel (λ i, i ∉ val_idxs) fr fr'⌝ ∗ *)
+(*         ⌜Forall2 (fun i v => f_locs fr' !! localimm i = Some v) val_localidxs vs_payload⌝ ∗ *)
+(*         ⌜val_idxs = seq (fe_wlocal_offset fe + length wl) (length wl_save)⌝ ∗ *)
+(*         ⌜val_localidxs = map prelude.W.Mk_localidx val_idxs⌝ *)
+(*         )%I). *)
+(*       iApply cwp_val_app; first done. *)
+(*       eapply cwp_save_stack_w in Hsave; eauto. *)
+(*       + destruct Hsave as (-> & -> & -> & Hsave). *)
+(*         iApply (Hsave with "[$] [$]"). *)
+(*         iIntros (f' [Hfsame Hfchanged]). *)
+(*         unfold fvs_combine. *)
+(*         auto. *)
+(*       + admit. (* easy pure conseqeunce of value_interp and *)
+(*       rep_values_interp, should be proved above the first wp_seq *)
+(*       rule *) *)
+(*     } *)
+(*     iIntros (fr_saved w) "(%val_idxs & -> & %Hfrel_fr_saved & %Hsaved & %Hval_idxs_seq & %Hval_localidxs) Hfr Hrun". *)
+(*     iAssert *)
+(*     (frame_interp rti sr se L (wl ++ wl_save ++ [prelude.W.T_i32] ++ wl_case_1 ++ wl_case_2  ++ wl_case_3 ++ wlf) fr_saved) *)
+(*       with "[Hframe]" as "Hframe_saved". *)
+(*     { admit. } (* TODO: Not really sure how to prove this. Definitely need helper lemma *) *)
+(**)
+(*     edestruct (util.nths_error_exists val_localidxs case_1_val_idxs vs_payload case_1_sum_locals (Forall2_length _ _ _ Hsaved)) as [case_1_vs_payload Hnerr_payload_c1]; try done. *)
+(**)
+(*     edestruct (util.nths_error_exists val_localidxs case_2_val_idxs vs_payload case_2_sum_locals (Forall2_length _ _ _ Hsaved)) as [case_2_vs_payload Hnerr_payload_c2]; try done. *)
+(**)
+(*     edestruct (util.nths_error_exists val_localidxs case_3_val_idxs vs_payload case_3_sum_locals (Forall2_length _ _ _ Hsaved)) as [case_3_vs_payload Hnerr_payload_c3]; try done. *)
+(**)
+(**)
+(*     iDestruct (frame_interp_wl_interp with "Hframe_saved") as "%Hwl_saved"; first done. *)
+(*     pose proof (interp_wl_length _ _ _ Hwl_saved) as Hfr_saved_locs_len. *)
+(**)
+(*     assert (tag_idx < length (f_locs fr_saved)) as Htag_in_fr_saved. *)
+(*     { *)
+(*       subst tag_idx. *)
+(*       simpl. *)
+(*       eapply Nat.lt_le_trans; last done. *)
+(*       - rewrite app_assoc. *)
+(*         subst fe. *)
+(*         instantiate (1 := F). *)
+(*         repeat rewrite length_app. *)
+(*         lias. *)
+(*     } *)
+(**)
+(*     (* Store tag *) *)
+(*     rewrite (app_assoc (map _ _)). *)
+(*     iApply (cwp_seq with "[Hfr Hrun]"). *)
+(*     { *)
+(*       instantiate (1 := λ fr' vs, ( *)
+(*         ⌜vs = []⌝ ∗ *)
+(*         ⌜frame_rel (λ j, j ≠ tag_idx) fr_saved fr'⌝ ∗ *)
+(*         ⌜f_locs fr' !! tag_idx = Some (VAL_int32 (Wasm_int.Int32.repr tag))⌝ *)
+(*         )%I). *)
+(*       iApply (cwp_local_set with "[] [$] [$]"); first done. *)
+(*       iSplit; first done. *)
+(*       iSplit. *)
+(*       - iPureIntro. *)
+(*         split; last done. *)
+(*         intros j Hneq. *)
+(*         simpl. *)
+(*         rewrite list_lookup_insert_ne; [reflexivity | lia]. *)
+(*       - iSimpl. *)
+(*         iPureIntro. *)
+(*         rewrite list_lookup_insert_eq; try done. *)
+(*     } *)
+(*     iIntros (fr_saved_and_tag w) "(-> & %Hfrel_fr_saved_and_tag & %Hsaved_and_tag) Hfr Hrun". *)
+(*     clear_nils. *)
+(**)
+(*     (* relate starting frame fr and fr_saved_and_tag *) *)
+(*     pose proof (frame_rel_mask_trans_combine _ _ _ _ _ Hfrel_fr_saved Hfrel_fr_saved_and_tag) as Hfrel_fr_and_fr_saved_and_tag. *)
+(*     simpl in Hfrel_fr_and_fr_saved_and_tag. *)
+(**)
+(*     assert (frame_rel lmask fr fr_saved_and_tag) as Hfrel_lmask_saved_and_tag. *)
+(*     { *)
+(*       eapply frame_rel_mask_mono; [| exact Hfrel_fr_and_fr_saved_and_tag]. *)
+(*       intros i [Hi_lo Hi_hi]. *)
+(*       split. *)
+(*       + rewrite Hval_idxs_seq. *)
+(*         intro Hin. apply elem_of_seq in Hin. lia. *)
+(*       + unfold tag_idx. rewrite length_app. lia. *)
+(*     } *)
+(*     pose proof Hfrel_fr_and_fr_saved_and_tag as [_ ->]. *)
+(*     iDestruct (labels_interp_mono _ _ _ _ fr_saved_and_tag _ _ _ _ with "Hlabels") as "Hlabels'"; first done. *)
+(*     { *)
+(*       instantiate (1 := (wlmask (fe_of_context F') (wl ++ wl_save ++ [prelude.W.T_i32]))). *)
+(*       intros i [Hi_lo Hi_hi]. *)
+(*       simpl. *)
+(*       split. *)
+(*       + exact Hi_lo. *)
+(*       + rewrite -fe_of_context_labels. *)
+(*         rewrite !length_app. simpl. *)
+(*         subst fe. *)
+(*         lia. *)
+(*     } *)
+(**)
+(*     assert (Forall2 (λ (i : prelude.W.localidx) (v : value), f_locs fr_saved_and_tag !! localimm i = Some v) *)
+(*       val_localidxs vs_payload) as Hfr_saved_and_tag_payload. *)
+(*     { *)
+(*       eapply forall2_lookup_same. *)
+(*       3: done. *)
+(*       - intros j Hneq. instantiate (1 := tag_idx) in Hneq. *)
+(*         destruct Hfrel_fr_saved_and_tag as [-> _]; done. *)
+(*       - subst val_idxs val_localidxs tag_idx. *)
+(*         rewrite length_app Nat.add_assoc. *)
+(*         apply map_seq_forall_localidx_neq. *)
+(*     } *)
+(**)
+(*     iAssert *)
+(*       (frame_interp rti sr se L (wl ++ wl_save ++ [prelude.W.T_i32] ++ wl_case_1 ++ wl_case_2 ++ wl_case_3 ++ wlf) fr_saved_and_tag) *)
+(*       with "[Hframe_saved]" as "Hframe_saved_and_tag". *)
+(*     { admit. } (* TODO: Not really sure how to prove this. Definitely need helper lemma *) *)
+(**)
+(*     (* Create defaults *) *)
+(*     iApply (cwp_seq with "[Hfr Hrun]"). *)
+(*     { *)
+(*       eapply cwp_create_defaults in Hcreate_defaults as (_ & _ & _ & Hcreate_defaults). *)
+(*       iDestruct (Hcreate_defaults with "[$] [$] []") as "Hcreate_defaults". *)
+(*       { *)
+(*         by instantiate (1 := λ f vs, (⌜f = fr_saved_and_tag⌝ ∗ ⌜vs = (map default_of_value_type wl_ret)⌝)%I). *)
+(*       } *)
+(*       iApply "Hcreate_defaults". *)
+(*     } *)
+(*     iIntros (??) "[-> ->] Hfr Hrun". *)
+(**)
+(*     (* Case analysis: Is tag 0 or 1 or 2? *) *)
+(**)
+(*     apply lookup_lt_Some in Htag_type_lookup as Hi. *)
+(*     destruct tag as [| [|[|]]]; last done. *)
+(**)
+(*     - (* Case: tag = 0 *) *)
+(*       (* -------- Case 1 -------- *) *)
+(*       rewrite (app_assoc (to_consts _)). *)
+(*       iApply (cwp_seq with "[-]"). *)
+(*       { *)
+(*         iApply (compat_case_block_success with "[] [$] [$] [$] [$] [$] [$] [$] [$] [$]"). *)
+(*         2: instantiate (1 := []). *)
+(*         all: clear_nils. *)
+(*         1, 2, 3, 4, 5, 6, 8, 9, 11, 13, 14: done. *)
+(*         4: iApply "Hsem_es1". *)
+(*         1: done. *)
+(*         1: by rewrite length_map. *)
+(*         by subst val_idxs. *)
+(*       } *)
+(*       iIntros (f_es_case_1 vs) "(_ & %Hlen_vs & %Hfrel_new & Hframe & %os & %θ' & Hos & Hvs & Hrt) Hfr Hrun". *)
+(**)
+(*       (* -------- Case 2 -------- *) *)
+(*       rewrite (app_assoc (to_consts _)). *)
+(*       iApply (cwp_seq with "[Hfr Hrun]"). *)
+(*       { *)
+(*         iApply (compat_case_block_fail with "[$] [$]"). *)
+(*         3: by instantiate (1 := 0). *)
+(*         2, 3, 4, 5: done. *)
+(*         rewrite -Hsaved_and_tag. *)
+(*         destruct Hfrel_new as [Hmask _]. *)
+(*         symmetry. *)
+(*         apply Hmask. *)
+(*         subst tag_idx fe. *)
+(*         unfold wlmask. *)
+(*         repeat rewrite length_app. *)
+(*         rewrite -fe_of_context_labels. *)
+(*         lias. *)
+(*       } *)
+(*       iIntros (??) "(-> & ->) Hfr Hrun". *)
+(**)
+(*       (* -------- Case 3 -------- *) *)
+(*       iApply (cwp_wand with "[Hfr Hrun]"). *)
+(*       { *)
+(*         iApply (compat_case_block_fail with "[$] [$]"). *)
+(*         3: by instantiate (1 := 0). *)
+(*         2, 3, 4, 5: done. *)
+(*         rewrite -Hsaved_and_tag. *)
+(*         destruct Hfrel_new as [Hmask _]. *)
+(*         symmetry. *)
+(*         apply Hmask. *)
+(*         subst tag_idx fe. *)
+(*         unfold wlmask. *)
+(*         repeat rewrite length_app. *)
+(*         rewrite -fe_of_context_labels. *)
+(*         lias. *)
+(*       } *)
+(*       iIntros (??) "(-> & ->)". *)
+(*       iFrame. *)
+(*       iPureIntro. *)
+(*       rewrite -fe_of_context_labels in Hfrel_new. *)
+(*       unfold lmask. *)
+(*       eapply frame_rel_trans. *)
+(*       + eapply frame_rel_mask_mono; [| exact Hfrel_lmask_saved_and_tag]. *)
+(*         intros i [Hi_lo Hi_hi]. unfold lmask, wlmask. split; exact Hi_lo || exact Hi_hi. *)
+(*       + eapply frame_rel_wlmask_mono; [| exact Hfrel_new]. *)
+(*         rewrite length_app. lia. *)
+(**)
+(*     - (* Case: tag = 1 *) *)
+(*       (* -------- Case 1 -------- *) *)
+(*       rewrite (app_assoc (to_consts _)). *)
+(*       iApply (cwp_seq with "[Hfr Hrun]"). *)
+(*       { *)
+(*         iApply (compat_case_block_fail with "[$] [$]"). *)
+(*         3: by instantiate (1 := 1). *)
+(*         1, 2, 3, 4: done. *)
+(*         by rewrite length_map. *)
+(*       } *)
+(*       iIntros (??) "(-> & ->) Hfr Hrun". *)
+(**)
+(*       iDestruct (labels_interp_mono _ _ _ _ fr_saved_and_tag _ _ _ _ with "Hlabels") as "Hlabels'''"; first done. *)
+(*       { *)
+(*         instantiate (1 := (wlmask (fe_of_context F') (wl ++ wl_save ++ [prelude.W.T_i32] ++ wl_case_1))). *)
+(*         intros i [Hi_lo Hi_hi]. *)
+(*         simpl. *)
+(*         split. *)
+(*         + exact Hi_lo. *)
+(*         + rewrite -fe_of_context_labels. *)
+(*           rewrite !length_app. simpl. *)
+(*           subst fe. *)
+(*           lia. *)
+(*       } *)
+(**)
+(*       (* -------- Case 2 -------- *) *)
+(*       rewrite (app_assoc (to_consts _)). *)
+(*       iApply (cwp_seq with "[-]"). *)
+(*       { *)
+(*         iApply (compat_case_block_success with "[] [$] [$] [$] [$] [$] [$] [$] [$] [$]"). *)
+(*         1, 2, 3, 4, 5, 6, 8, 9, 11, 13, 14: done. *)
+(*         4: iApply "Hsem_es2". *)
+(*         1: done. *)
+(*         1: by rewrite length_map. *)
+(*         by subst val_idxs. *)
+(*       } *)
+(*       iIntros (f_es_case_2 vs) "(_ & %Hlen_vs & %Hfrel_new & Hframe & %os & %θ' & Hos & Hvs & Hrt) Hfr Hrun". *)
+(**)
+(*       (* -------- Case 3 -------- *) *)
+(*       iApply (cwp_wand with "[Hfr Hrun]"). *)
+(*       { *)
+(*         iApply (compat_case_block_fail with "[$] [$]"). *)
+(*         3: by instantiate (1 := 1). *)
+(*         2, 3, 4, 5: done. *)
+(*         rewrite -Hsaved_and_tag. *)
+(*         destruct Hfrel_new as [Hmask _]. *)
+(*         symmetry. *)
+(*         apply Hmask. *)
+(*         subst tag_idx fe. *)
+(*         unfold wlmask. *)
+(*         repeat rewrite length_app. *)
+(*         rewrite -fe_of_context_labels. *)
+(*         lias. *)
+(*       } *)
+(*       iIntros (??) "(-> & ->)". *)
+(*       iFrame. *)
+(*       iPureIntro. *)
+(*       rewrite -fe_of_context_labels in Hfrel_new. *)
+(*       unfold lmask. *)
+(*       eapply frame_rel_trans. *)
+(*       + eapply frame_rel_mask_mono; [| exact Hfrel_lmask_saved_and_tag]. *)
+(*         intros i [Hi_lo Hi_hi]. unfold lmask, wlmask. split; exact Hi_lo || exact Hi_hi. *)
+(*       + eapply frame_rel_wlmask_mono; [| exact Hfrel_new]. *)
+(*         rewrite length_app. lia. *)
+(**)
+(*     - (* Case: tag = 2 *) *)
+(*       (* -------- Case 1 -------- *) *)
+(*       rewrite (app_assoc (to_consts _)). *)
+(*       iApply (cwp_seq with "[Hfr Hrun]"). *)
+(*       { *)
+(*         iApply (compat_case_block_fail with "[$] [$]"). *)
+(*         3: by instantiate (1 := 2). *)
+(*         1, 2, 3, 4: done. *)
+(*         by rewrite length_map. *)
+(*       } *)
+(*       iIntros (??) "(-> & ->) Hfr Hrun". *)
+(**)
+(*       (* -------- Case 2 -------- *) *)
+(*       rewrite (app_assoc (to_consts _)). *)
+(*       iApply (cwp_seq with "[Hfr Hrun]"). *)
+(*       { *)
+(*         iApply (compat_case_block_fail with "[$] [$]"). *)
+(*         3: by instantiate (1 := 2). *)
+(*         1, 2, 3, 4 : done. *)
+(*         by rewrite length_map. *)
+(*       } *)
+(*       iIntros (??) "(-> & ->) Hfr Hrun". *)
+(**)
+(*       iDestruct (labels_interp_mono _ _ _ _ fr_saved_and_tag _ _ _ _ with "Hlabels") as "Hlabels'''"; first done. *)
+(*       { *)
+(*         instantiate (1 := (wlmask (fe_of_context F') (wl ++ wl_save ++ [prelude.W.T_i32] ++ wl_case_1 ++ wl_case_2))). *)
+(*         intros i [Hi_lo Hi_hi]. *)
+(*         simpl. *)
+(*         split. *)
+(*         + exact Hi_lo. *)
+(*         + rewrite -fe_of_context_labels. *)
+(*           rewrite !length_app. simpl. *)
+(*           subst fe. *)
+(*           lia. *)
+(*       } *)
+(**)
+(*       (* -------- Case 3 -------- *) *)
+(*       iApply (cwp_wand with "[-]"). *)
+(*       { *)
+(*         iApply (compat_case_block_success with "[] [$] [$] [$] [$] [$] [$] [$] [$] [$]"). *)
+(*         1, 2, 3, 4, 5, 6, 8, 9, 11, 13, 14: done. *)
+(*         4: iApply "Hsem_es3". *)
+(*         1: done. *)
+(*         1: by rewrite length_map. *)
+(*         by subst val_idxs. *)
+(*       } *)
+(*       iIntros (f_es_case_3 vs) "(_ & %Hlen_vs & %Hfrel_new & Hframe & %os & %θ' & Hos & Hvs & Hrt)". *)
+(*       iFrame. *)
+(*       iPureIntro. *)
+(*       rewrite -fe_of_context_labels in Hfrel_new. *)
+(*       unfold lmask. *)
+(*       eapply frame_rel_trans. *)
+(*       + eapply frame_rel_mask_mono; [| exact Hfrel_lmask_saved_and_tag]. *)
+(*         intros i [Hi_lo Hi_hi]. unfold lmask, wlmask. split; exact Hi_lo || exact Hi_hi. *)
+(*       + eapply frame_rel_wlmask_mono; [| exact Hfrel_new]. *)
+(*         rewrite length_app. lia. *)
+(*   Admitted. *)
 
-    (* TODO: we should also know that tag < length (ρs_sum). This will follow easily from the above and Htag_type_lookup *)
-
-    iDestruct (big_sepL2_length with "Hrvs") as "%Hlen".
-    destruct vs as [|v_tag vs_payload]; first inversion Hlen.
-    clear Hlen.
-    iDestruct (atoms_interp_cons with "Hrvs") as "[-> Hatoms_interp_payload]".
-
-    iPoseProof (frame_interp_wl_interp with "Hframe") as "%Hwl"; first done.
-    rewrite list_extra.cons_app in Hhas_values.
-    apply has_values_app_inv in Hhas_values as (e_tag & es_payload & -> & Hhv_tag & Hhvs_payload).
-
-    (* save payload *)
-    rewrite (app_assoc (e_tag ++ _)).
-    iApply (cwp_seq with "[Hfr Hrun]").
-    {
-      rewrite <- (app_assoc e_tag).
-      instantiate (1 := λ fr' vs, (
-        ∃ val_idxs,
-        ⌜vs = [VAL_int32 (Wasm_int.Int32.repr tag)]⌝ ∗
-        ⌜frame_rel (λ i, i ∉ val_idxs) fr fr'⌝ ∗
-        ⌜Forall2 (fun i v => f_locs fr' !! localimm i = Some v) val_localidxs vs_payload⌝ ∗
-        ⌜val_idxs = seq (fe_wlocal_offset fe + length wl) (length wl_save)⌝ ∗
-        ⌜val_localidxs = map prelude.W.Mk_localidx val_idxs⌝
-        )%I).
-      iApply cwp_val_app; first done.
-      eapply cwp_save_stack_w in Hsave; eauto.
-      + destruct Hsave as (-> & -> & -> & Hsave).
-        iApply (Hsave with "[$] [$]").
-        iIntros (f' [Hfsame Hfchanged]).
-        unfold fvs_combine.
-        auto.
-      + admit. (* easy pure conseqeunce of value_interp and
-      rep_values_interp, should be proved above the first wp_seq
-      rule *)
-    }
-    iIntros (fr_saved w) "(%val_idxs & -> & %Hfrel_fr_saved & %Hsaved & %Hval_idxs_seq & %Hval_localidxs) Hfr Hrun".
-    iAssert
-      (frame_interp rti sr se L (wl ++ wl_save ++ [prelude.W.T_i32] ++ wl_case_1 ++ wl_case_2 ++ wlf) fr_saved)
-      with "[Hframe]" as "Hframe_saved".
-    { admit. } (* TODO: Not really sure how to prove this. Definitely need helper lemma *)
-
-    edestruct (util.nths_error_exists val_localidxs case_1_val_idxs vs_payload case_1_sum_locals (Forall2_length _ _ _ Hsaved)) as [case_1_vs_payload Hnerr_payload_c1]; try done.
-
-    edestruct (util.nths_error_exists val_localidxs case_2_val_idxs vs_payload case_2_sum_locals (Forall2_length _ _ _ Hsaved)) as [case_2_vs_payload Hnerr_payload_c2]; try done.
-
-    iDestruct (frame_interp_wl_interp with "Hframe_saved") as "%Hwl_saved"; first done.
-    pose proof (interp_wl_length _ _ _ Hwl_saved) as Hfr_saved_locs_len.
-
-    assert (tag_idx < length (f_locs fr_saved)) as Htag_in_fr_saved.
-    {
-      subst tag_idx.
-      simpl.
-      eapply Nat.lt_le_trans; last done.
-      - rewrite app_assoc.
-        subst fe.
-        instantiate (1 := F).
-        repeat rewrite length_app.
-        lias.
-    }
-
-    (* Store tag *)
-    rewrite (app_assoc (map _ _)).
-    iApply (cwp_seq with "[Hfr Hrun]").
-    {
-      instantiate (1 := λ fr' vs, (
-        ⌜vs = []⌝ ∗
-        ⌜frame_rel (λ j, j ≠ tag_idx) fr_saved fr'⌝ ∗
-        ⌜f_locs fr' !! tag_idx = Some (VAL_int32 (Wasm_int.Int32.repr tag))⌝
-        )%I).
-      iApply (cwp_local_set with "[] [$] [$]"); first done.
-      iSplit; first done.
-      iSplit.
-      - iPureIntro.
-        split; last done.
-        intros j Hneq.
-        simpl.
-        rewrite list_lookup_insert_ne; [reflexivity | lia].
-      - iSimpl.
-        iPureIntro.
-        rewrite list_lookup_insert_eq; try done.
-    }
-    iIntros (fr_saved_and_tag w) "(-> & %Hfrel_fr_saved_and_tag & %Hsaved_and_tag) Hfr Hrun".
-    clear_nils.
-
-    (* relate starting frame fr and fr_saved_and_tag *)
-    pose proof (frame_rel_mask_trans_combine _ _ _ _ _ Hfrel_fr_saved Hfrel_fr_saved_and_tag) as Hfrel_fr_and_fr_saved_and_tag.
-    simpl in Hfrel_fr_and_fr_saved_and_tag.
-
-    assert (frame_rel lmask fr fr_saved_and_tag) as Hfrel_lmask_saved_and_tag.
-    {
-      eapply frame_rel_mask_mono; [| exact Hfrel_fr_and_fr_saved_and_tag].
-      intros i [Hi_lo Hi_hi].
-      split.
-      + rewrite Hval_idxs_seq.
-        intro Hin. apply elem_of_seq in Hin. lia.
-      + unfold tag_idx. rewrite length_app. lia.
-    }
-    pose proof Hfrel_fr_and_fr_saved_and_tag as [_ ->].
-    iDestruct (labels_interp_mono _ _ _ _ fr_saved_and_tag _ _ _ _ with "Hlabels") as "Hlabels'"; first done.
-    {
-      instantiate (1 := (wlmask (fe_of_context F') (wl ++ wl_save ++ [prelude.W.T_i32]))).
-      intros i [Hi_lo Hi_hi].
-      simpl.
-      split.
-      + exact Hi_lo.
-      + rewrite -fe_of_context_labels.
-        rewrite !length_app. simpl.
-        subst fe.
-        lia.
-    }
-
-    assert (Forall2 (λ (i : prelude.W.localidx) (v : value), f_locs fr_saved_and_tag !! localimm i = Some v)
-      val_localidxs vs_payload) as Hfr_saved_and_tag_payload.
-    {
-      eapply forall2_lookup_same.
-      3: done.
-      - intros. instantiate (1 := tag_idx) in H.
-        destruct Hfrel_fr_saved_and_tag as [-> _]; done.
-      - subst val_idxs val_localidxs tag_idx.
-        rewrite length_app Nat.add_assoc.
-        apply map_seq_forall_localidx_neq.
-    }
-
-    iAssert
-      (frame_interp rti sr se L (wl ++ wl_save ++ [prelude.W.T_i32] ++ wl_case_1 ++ wl_case_2 ++ wlf) fr_saved_and_tag)
-      with "[Hframe_saved]" as "Hframe_saved_and_tag".
-    { admit. } (* TODO: Not really sure how to prove this. Definitely need helper lemma *)
-
-    (* Create defaults *)
-    iApply (cwp_seq with "[Hfr Hrun]").
-    {
-      eapply cwp_create_defaults in Hcreate_defaults as (_ & _ & _ & Hcreate_defaults).
-      iDestruct (Hcreate_defaults with "[$] [$] []") as "Hcreate_defaults".
-      {
-        by instantiate (1 := λ f vs, (⌜f = fr_saved_and_tag⌝ ∗ ⌜vs = (map default_of_value_type wl_ret)⌝)%I).
-      }
-      iApply "Hcreate_defaults".
-    }
-    iIntros (??) "[-> ->] Hfr Hrun".
-
-    (* Case analysis: Is tag 0 or 1? *)
-
-    apply lookup_lt_Some in Htag_type_lookup as Hi.
-    destruct tag as [| [|]]; last done.
-
-    - (* Case: tag = 0 *)
-      (* -------- Case 1 -------- *)
-      rewrite (app_assoc (to_consts _)).
-      iApply (cwp_seq with "[-]").
-      {
-        iApply (compat_case_block_success with "[] [$] [$] [$] [$] [$] [$] [$] [$] [$]").
-        2: instantiate (1 := []).
-        all: clear_nils.
-        1, 2, 3, 4, 5, 6, 8, 9, 11, 13, 14: done.
-        4: iApply "Hsem_es1".
-        1: done.
-        1: by rewrite length_map.
-        by subst val_idxs.
-      }
-      iIntros (f_es_case_1 vs) "(_ & %Hlen_vs & %Hfrel_new & Hframe & %os & %θ' & Hos & Hvs & Hrt) Hfr Hrun".
-
-      (* -------- Case 2 -------- *)
-      iApply (cwp_wand with "[Hfr Hrun]").
-      {
-        iApply (compat_case_block_fail with "[$] [$]").
-        2, 3, 4, 5, 6, 9, 10: done.
-        2: by instantiate (1 := 0).
-        2: done.
-        rewrite -Hsaved_and_tag.
-        destruct Hfrel_new as [Hmask _].
-        symmetry.
-        apply Hmask.
-        subst tag_idx fe.
-        unfold wlmask.
-        repeat rewrite length_app.
-        rewrite -fe_of_context_labels.
-        lias.
-      }
-      (* iIntros (??) "(-> & ->) Hfr Hrun". *)
-      (* TODO: we would probably want fr and run resource back from the block_fail lemma *)
-      iIntros (??) "(-> & ->)".
-      iFrame.
-      iPureIntro.
-      rewrite -fe_of_context_labels in Hfrel_new.
-      unfold lmask.
-      eapply frame_rel_trans.
-      + eapply frame_rel_mask_mono; [| exact Hfrel_lmask_saved_and_tag].
-        intros i [Hi_lo Hi_hi]. unfold lmask, wlmask. split; exact Hi_lo || exact Hi_hi.
-      + eapply frame_rel_wlmask_mono; [| exact Hfrel_new].
-        rewrite length_app. lia.
-
-    - (* Case: tag = 1 *)
-      (* -------- Case 1 -------- *)
-      rewrite (app_assoc (to_consts _)).
-      iApply (cwp_seq with "[Hfr Hrun]").
-      {
-        iApply (compat_case_block_fail with "[$] [$]").
-        7: by instantiate (1 := 1).
-        2: instantiate (1 := []).
-        1, 2, 3, 4, 5, 6, 7, 8: done.
-        by rewrite length_map.
-      }
-      iIntros (??) "(-> & ->) Hfr Hrun".
-
-      iDestruct (labels_interp_mono _ _ _ _ fr_saved_and_tag _ _ _ _ with "Hlabels") as "Hlabels'''"; first done.
-      {
-        instantiate (1 := (wlmask (fe_of_context F') (wl ++ wl_save ++ [prelude.W.T_i32] ++ wl_case_1))).
-        intros i [Hi_lo Hi_hi].
-        simpl.
-        split.
-        + exact Hi_lo.
-        + rewrite -fe_of_context_labels.
-          rewrite !length_app. simpl.
-          subst fe.
-          lia.
-      }
-
-      (* -------- Case 2 -------- *)
-      iApply (cwp_wand with "[-]").
-      {
-        iApply (compat_case_block_success with "[] [$] [$] [$] [$] [$] [$] [$] [$] [$]").
-        1, 2, 3, 4, 5, 6, 8, 9, 11, 13, 14, 15: done.
-        1: done.
-        1: by rewrite length_map.
-        by subst val_idxs.
-      }
-      iIntros (f_es_case_2 vs) "(_ & %Hlen_vs & %Hfrel_new & Hframe & %os & %θ' & Hos & Hvs & Hrt)".
-      iFrame.
-      iPureIntro.
-      rewrite -fe_of_context_labels in Hfrel_new.
-      unfold lmask.
-      eapply frame_rel_trans.
-      + eapply frame_rel_mask_mono; [| exact Hfrel_lmask_saved_and_tag].
-        intros i [Hi_lo Hi_hi]. unfold lmask, wlmask. split; exact Hi_lo || exact Hi_hi.
-      + eapply frame_rel_wlmask_mono; [| exact Hfrel_new].
-        rewrite length_app. lia.
-  Admitted.
-
-
-  Lemma compat_ternary_case M F L L' wt wt' wtf wl wl' wlf es' ess es1 es2 es3 τs τ1 τ2 τ3 τs' κ :
-    ess = [es1; es2; es3] ->
-    τs = [τ1; τ2; τ3] ->
-    let fe := fe_of_context F in
-    let WT := wt ++ wt' ++ wtf in
-    let WL := wl ++ wl' ++ wlf in
-    let lmask := wlmask fe wl in
-    let F' := F <| fc_labels ::= cons (τs', L') |> in
-    let ψ := InstrT [SumT κ τs] τs' in
-    Forall2
-      (fun τ es =>
-         (forall wt wt' wtf wl wl' wlf es',
-            let fe' := fe_of_context F' in
-            let WT := wt ++ wt' ++ wtf in
-            let WL := wl ++ wl' ++ wlf in
-            let lmask := wlmask fe' wl in
-            run_codegen (compile_instrs mr fe' es) wt wl = inr ((), wt', wl', es') ->
-            ⊢ have_instr_type_sem rti sr mr M F' L WT WL lmask es' (InstrT [τ] τs') L'))
-      τs ess ->
-    has_instruction_type_ok F ψ L' ->
-    run_codegen (compile_instr mr fe (ICase ψ L' ess)) wt wl = inr ((), wt', wl', es') ->
-    ⊢ have_instr_type_sem rti sr mr M F L WT WL lmask es' ψ L'.
-Proof.
-    intros -> -> fe WT WL lmask F' Ψ Hforall Hok Hcg.
-    set (τs := [τ1; τ2; τ3]).
-    rewrite Forall2_cons_iff in Hforall.
-    destruct Hforall as [Hes1 H2].
-    rewrite Forall2_cons_iff in H2.
-    destruct H2 as [Hes2 H3].
-    rewrite Forall2_cons_iff in H3.
-    destruct H3 as [Hes3 _].
-    subst Ψ.
-    cbn [compile_instr] in Hcg.
-    destruct κ as [ ρ rf | ]; last inversion Hcg.
-    destruct ρ  as [ | ρs_sum | | ]; try done.
-    destruct τs' as [ | τ_res τs' ]; first done.
-    destruct τs'; last done.
-
-    inv_cg_bind Hcg wl_ret ?wt ?wt ?wl ?wl ?es ?es Hres_type Hcg.
-    inv_cg_try_option Hres_type; subst.
-
-    destruct (Wasm_int.Int32.modulus <? length ρs_sum)%Z eqn:Hcmp; first inversion Hcg.
-    inv_cg_bind Hcg ?units ?wt ?wt ?wl ?wl ?es es_case1 Hret Hcg.
-    inv_cg_ret Hret; subst.
-    apply Z.ltb_ge in Hcmp.
-
-    inv_cg_bind Hcg ρs_atom ?wt ?wt ?wl ?wl ?es ?es Hιs Hcg.
-    inv_cg_try_option Hιs; subst.
-    inv_cg_bind Hcg val_localidxs wt_save ?wt wl_save ?wl es_save ?es Hsave Hcg.
-    repeat rewrite app_nil_r in Hsave.
-
-    (* Save tag *)
-    inv_cg_bind Hcg tag_localidx ?wt ?wt ?wl ?wl ?es ?es HsaveTag Hcg.
-    unfold save_stack1 in HsaveTag.
-    inv_cg_bind HsaveTag ?tl ?wt ?wt ?wl ?wl ?es ?es Halloc_tag HsaveTag.
-    apply wp_wlalloc in Halloc_tag as [Hlocal_tag_idx [-> [-> ->]]].
-    inv_cg_bind HsaveTag [] ?wt ?wt ?wl ?wl es_set_tag ?es HsetTag HretTagIdx.
-    inv_cg_emit HsetTag; subst.
-    inv_cg_ret HretTagIdx; subst.
-
-    clear_nils.
-    set (tag_idx := (fe_wlocal_offset fe + length (wl ++ wl_save))).
-    set (tag_localidx := Mk_localidx tag_idx).
-    replace (Mk_localidx (fe_wlocal_offset fe + length (wl ++ wl_save))) with tag_localidx in *; last done.
-
-    (* Put default result values on stack *)
-    inv_cg_bind Hcg [] ?wt ?wt ?wl ?wl es_create_defaults ?es Hcreate_defaults Hcg.
-    apply run_codegen_create_defaults in Hcreate_defaults as H.
-    destruct H as (_ & -> & -> & _).
-
-    (* Case blocks *)
-    cbv [map length seq zip Datatypes.uncurry] in Hcg.
-
-    clear_nils.
-
-    inv_cg_bind Hcg [] ?wt ?wt ?wl ?wl ?es es_case2 Hcase_es1 Hcases.
-    inv_cg_bind Hcases [] ?wt ?wt ?wl ?wl ?es ?es Hcase_es2 Hcase_es3.
-
-    (* Case es1 *)
-
-    inv_cg_bind Hcase_es1 ?pair ?wt ?wt ?wl ?wl ?es ?es Hcase_es1 Hcase_es1_block.
-    destruct pair, u.
-    inv_cg_emit Hcase_es1_block; subst.
-    apply run_codegen_capture in Hcase_es1 as [Hcase_es1 ->].
-
-    inv_cg_bind Hcase_es1 [] ?wt ?wt ?wl ?wl ?es ?es Hget_tag Hcase_es1.
-    inv_cg_emit Hget_tag; subst.
-
-    inv_cg_bind Hcase_es1 [] ?wt ?wt ?wl ?wl ?es ?es Htag0 Hcase_es1.
-    inv_cg_emit Htag0; subst.
-
-    inv_cg_bind Hcase_es1 [] ?wt ?wt ?wl ?wl ?es ?es Hcompare_tag Hcase_es1.
-    inv_cg_emit Hcompare_tag; subst.
-
-    inv_cg_bind Hcase_es1 [] ?wt ?wt ?wl ?wl ?es ?es Hbr_case Hcase_es1.
-    inv_cg_emit Hbr_case; subst.
-
-    inv_cg_bind Hcase_es1 [] ?wt ?wt ?wl ?wl es_drop_1 ?es Hdrop_consts_1 Hcase_es1.
-    apply run_codegen_drop_consts in Hdrop_consts_1 as H.
-    destruct H as (_ & -> & -> & _).
-
-    inv_cg_bind Hcase_es1 ρ_case1 ?wt ?wt ?wl ?wl ?es ?es Hlookup Hcase_es1.
-    inv_cg_try_option Hlookup; subst.
-
-    inv_cg_bind Hcase_es1 case_1_sum_locals ?wt ?wt ?wl ?wl ?es ?es Hinject Hcase_es1.
-    inv_cg_try_option Hinject; subst.
-
-    inv_cg_bind Hcase_es1 [] ?wt wt_case_1 ?wl wl_case_1 ?es es_case_1 Hget_locals_1 Hcase_es1.
-    inv_cg_bind Hget_locals_1 case_1_val_idxs ?wt wt_get_locals_1 ?wl wl_get_locals_1 ?es es_get_locals_1 Hnths_error Hget_locals_1.
-    inv_cg_try_option Hnths_error; subst.
-
-    destruct (run_codegen_get_locals _ _ _ _ _ _ _ Hget_locals_1) as ([] & -> & ->).
-
-    clear_nils.
-
-    (* Case es2 *)
-
-    inv_cg_bind Hcase_es2 ?pair ?wt ?wt ?wl ?wl ?es ?es Hcase_es2 Hcase_es2_block.
-    destruct pair, u.
-    inv_cg_emit Hcase_es2_block; subst.
-    apply run_codegen_capture in Hcase_es2 as [Hcase_es2 ->].
-
-    inv_cg_bind Hcase_es2 [] ?wt ?wt ?wl ?wl ?es ?es Hget_tag Hcase_es2.
-    inv_cg_emit Hget_tag; subst.
-
-    inv_cg_bind Hcase_es2 [] ?wt ?wt ?wl ?wl ?es ?es Htag0 Hcase_es2.
-    inv_cg_emit Htag0; subst.
-
-    inv_cg_bind Hcase_es2 [] ?wt ?wt ?wl ?wl ?es ?es Hcompare_tag Hcase_es2.
-    inv_cg_emit Hcompare_tag; subst.
-
-    inv_cg_bind Hcase_es2 [] ?wt ?wt ?wl ?wl ?es ?es Hbr_case Hcase_es2.
-    inv_cg_emit Hbr_case; subst.
-
-    inv_cg_bind Hcase_es2 [] ?wt ?wt ?wl ?wl es_drop_2 ?es Hdrop_consts_2 Hcase_es2.
-    apply run_codegen_drop_consts in Hdrop_consts_2 as H.
-    destruct H as (_ & -> & -> & _).
-
-    inv_cg_bind Hcase_es2 ρ_case2 ?wt ?wt ?wl ?wl ?es ?es Hlookup Hcase_es2.
-    inv_cg_try_option Hlookup; subst.
-
-    inv_cg_bind Hcase_es2 case_2_sum_locals ?wt ?wt ?wl ?wl ?es ?es Hinject Hcase_es2.
-    inv_cg_try_option Hinject; subst.
-
-    inv_cg_bind Hcase_es2 [] ?wt wt_case_2 ?wl wl_case_2 ?es es_case_2 Hget_locals_2 Hcase_es2.
-    inv_cg_bind Hget_locals_2 case_2_val_idxs ?wt wt_get_locals_2 ?wl wl_get_locals_2 ?es es_get_locals_2 Hnths_error Hget_locals_2.
-    inv_cg_try_option Hnths_error; subst.
-
-    destruct (run_codegen_get_locals _ _ _ _ _ _ _ Hget_locals_2) as ([] & -> & ->).
-
-
-    (* Case es3 *)
-    inv_cg_bind Hcase_es3 ?units ?wt ?wt ?wl ?wl ?es ?es Hcase_es3 Hmret.
-    inv_cg_ret Hmret; subst.
-
-    inv_cg_bind Hcase_es3 ?pair ?wt ?wt ?wl ?wl ?es ?es Hcase_es3 Hcase_es3_block.
-    destruct pair, u.
-    inv_cg_emit Hcase_es3_block; subst.
-    apply run_codegen_capture in Hcase_es3 as [Hcase_es3 ->].
-
-    inv_cg_bind Hcase_es3 [] ?wt ?wt ?wl ?wl ?es ?es Hget_tag Hcase_es3.
-    inv_cg_emit Hget_tag; subst.
-
-    inv_cg_bind Hcase_es3 [] ?wt ?wt ?wl ?wl ?es ?es Htag0 Hcase_es3.
-    inv_cg_emit Htag0; subst.
-
-    inv_cg_bind Hcase_es3 [] ?wt ?wt ?wl ?wl ?es ?es Hcompare_tag Hcase_es3.
-    inv_cg_emit Hcompare_tag; subst.
-
-    inv_cg_bind Hcase_es3 [] ?wt ?wt ?wl ?wl ?es ?es Hbr_case Hcase_es3.
-    inv_cg_emit Hbr_case; subst.
-
-    inv_cg_bind Hcase_es3 [] ?wt ?wt ?wl ?wl es_drop_3 ?es Hdrop_consts_3 Hcase_es3.
-    apply run_codegen_drop_consts in Hdrop_consts_3 as H.
-    destruct H as (_ & -> & -> & _).
-
-    inv_cg_bind Hcase_es3 ρ_case3 ?wt ?wt ?wl ?wl ?es ?es Hlookup Hcase_es3.
-    inv_cg_try_option Hlookup; subst.
-
-    inv_cg_bind Hcase_es3 case_3_sum_locals ?wt ?wt ?wl ?wl ?es ?es Hinject Hcase_es3.
-    inv_cg_try_option Hinject; subst.
-
-    inv_cg_bind Hcase_es3 [] ?wt wt_case_3 ?wl wl_case_3 ?es es_case_3 Hget_locals_3 Hcase_es3.
-    inv_cg_bind Hget_locals_3 case_3_val_idxs ?wt wt_get_locals_3 ?wl wl_get_locals_3 ?es es_get_locals_3 Hnths_error Hget_locals_3.
-    inv_cg_try_option Hnths_error; subst.
-
-    destruct (run_codegen_get_locals _ _ _ _ _ _ _ Hget_locals_3) as ([] & -> & ->).
-
-
-    (* clean up *)
-    subst WT WL.
-    clear_nils.
-    simplify_eq.
-
-    (* Iris Proof *)
-    iIntros (? ? ? ? ? ? ? ?) "%Hsem %Hhas_values #Hinst #Hlabels #Hreturn Hrvs Hvs Hframe Hrt Hfr Hrun".
-    iDestruct (Hes1 _ _ (wt_case_2 ++ wt_case_3 ++ wtf) _ _ (wl_case_2 ++ wl_case_3 ++ wlf) _ Hcase_es1) as "Hsem_es1".
-    iDestruct (Hes2 _ _ (wt_case_3 ++ wtf) _ _ (wl_case_3 ++ wlf) _ Hcase_es2) as "Hsem_es2".
-    iDestruct (Hes3 _ _ (wtf) _ _ (wlf) _ Hcase_es3) as "Hsem_es3".
-
-    (* Our values are in the value interpretation for our specific SumT *)
-    (* This means that the values represent the tag and the payload. *)
-    iDestruct (values_interp_one_eq with "Hvs") as "Hvs".
-    iDestruct (value_interp_eq with "Hvs") as "Hvs".
-    unfold value_interp0, value_se_interp0.
-    iDestruct "Hvs" as "(%κ & %Hkind_sum & Hskind_as_type & Hsum_interp)".
-    (*unfold type_skind in Hkind_sum.*)
-    iDestruct "Hsum_interp" as (tag os' os_tag τ_tag ιs ιs_tag ixs  HSAtoms Htag_type_lookup Htag_type_arep Heval_rep_tail Hinject_sum_arep Hos'_ixs) "Hvalue_interp_os_i".
-    (*assert (os = I32A (Wasm_int.int_of_Z i32m i) :: os0) as ->; first by inversion HSAtoms.*)
-    simplify_eq.
-
-    apply lookup_lt_Some in Htag_type_lookup as Htag_size_bound.
-    assert (length τs = length ρs_sum) as Htyp_rep_len.
-    {
-      inversion Hok; subst.
-      unfold has_mono_rep_instr in H.
-      destruct H as [H _].
-      simpl in H.
-      rewrite Forall_singleton in H.
-      inversion H; subst.
-      inversion H1; subst.
-      apply has_kind_SumT_inv in H3 as (rf' & HF2).
-      by eapply Forall2_length.
-    }
-    assert (tag < Wasm_int.Int32.modulus)%Z as Htag_in_i32_bound.
-    { rewrite Htyp_rep_len in Htag_size_bound. eapply Z.lt_le_trans; last done. by apply Nat2Z.inj_lt. }
-
-    iDestruct (big_sepL2_length with "Hrvs") as "%Hlen".
-    destruct vs as [|v_tag vs_payload]; first inversion Hlen.
-    clear Hlen.
-    iDestruct (atoms_interp_cons with "Hrvs") as "[-> Hatoms_interp_payload]".
-
-    iPoseProof (frame_interp_wl_interp with "Hframe") as "%Hwl"; first done.
-    rewrite list_extra.cons_app in Hhas_values.
-    apply has_values_app_inv in Hhas_values as (e_tag & es_payload & -> & Hhv_tag & Hhvs_payload).
-
-    (* save payload *)
-    rewrite (app_assoc (e_tag ++ _)).
-    iApply (cwp_seq with "[Hfr Hrun]").
-    {
-      rewrite <- (app_assoc e_tag).
-      instantiate (1 := λ fr' vs, (
-        ∃ val_idxs,
-        ⌜vs = [VAL_int32 (Wasm_int.Int32.repr tag)]⌝ ∗
-        ⌜frame_rel (λ i, i ∉ val_idxs) fr fr'⌝ ∗
-        ⌜Forall2 (fun i v => f_locs fr' !! localimm i = Some v) val_localidxs vs_payload⌝ ∗
-        ⌜val_idxs = seq (fe_wlocal_offset fe + length wl) (length wl_save)⌝ ∗
-        ⌜val_localidxs = map prelude.W.Mk_localidx val_idxs⌝
-        )%I).
-      iApply cwp_val_app; first done.
-      eapply cwp_save_stack_w in Hsave; eauto.
-      + destruct Hsave as (-> & -> & -> & Hsave).
-        iApply (Hsave with "[$] [$]").
-        iIntros (f' [Hfsame Hfchanged]).
-        unfold fvs_combine.
-        auto.
-      + admit. (* easy pure conseqeunce of value_interp and
-      rep_values_interp, should be proved above the first wp_seq
-      rule *)
-    }
-    iIntros (fr_saved w) "(%val_idxs & -> & %Hfrel_fr_saved & %Hsaved & %Hval_idxs_seq & %Hval_localidxs) Hfr Hrun".
-    iAssert
-    (frame_interp rti sr se L (wl ++ wl_save ++ [prelude.W.T_i32] ++ wl_case_1 ++ wl_case_2  ++ wl_case_3 ++ wlf) fr_saved)
-      with "[Hframe]" as "Hframe_saved".
-    { admit. } (* TODO: Not really sure how to prove this. Definitely need helper lemma *)
-
-    edestruct (util.nths_error_exists val_localidxs case_1_val_idxs vs_payload case_1_sum_locals (Forall2_length _ _ _ Hsaved)) as [case_1_vs_payload Hnerr_payload_c1]; try done.
-
-    edestruct (util.nths_error_exists val_localidxs case_2_val_idxs vs_payload case_2_sum_locals (Forall2_length _ _ _ Hsaved)) as [case_2_vs_payload Hnerr_payload_c2]; try done.
-
-    edestruct (util.nths_error_exists val_localidxs case_3_val_idxs vs_payload case_3_sum_locals (Forall2_length _ _ _ Hsaved)) as [case_3_vs_payload Hnerr_payload_c3]; try done.
-
-
-    iDestruct (frame_interp_wl_interp with "Hframe_saved") as "%Hwl_saved"; first done.
-    pose proof (interp_wl_length _ _ _ Hwl_saved) as Hfr_saved_locs_len.
-
-    assert (tag_idx < length (f_locs fr_saved)) as Htag_in_fr_saved.
-    {
-      subst tag_idx.
-      simpl.
-      eapply Nat.lt_le_trans; last done.
-      - rewrite app_assoc.
-        subst fe.
-        instantiate (1 := F).
-        repeat rewrite length_app.
-        lias.
-    }
-
-    (* Store tag *)
-    rewrite (app_assoc (map _ _)).
-    iApply (cwp_seq with "[Hfr Hrun]").
-    {
-      instantiate (1 := λ fr' vs, (
-        ⌜vs = []⌝ ∗
-        ⌜frame_rel (λ j, j ≠ tag_idx) fr_saved fr'⌝ ∗
-        ⌜f_locs fr' !! tag_idx = Some (VAL_int32 (Wasm_int.Int32.repr tag))⌝
-        )%I).
-      iApply (cwp_local_set with "[] [$] [$]"); first done.
-      iSplit; first done.
-      iSplit.
-      - iPureIntro.
-        split; last done.
-        intros j Hneq.
-        simpl.
-        rewrite list_lookup_insert_ne; [reflexivity | lia].
-      - iSimpl.
-        iPureIntro.
-        rewrite list_lookup_insert_eq; try done.
-    }
-    iIntros (fr_saved_and_tag w) "(-> & %Hfrel_fr_saved_and_tag & %Hsaved_and_tag) Hfr Hrun".
-    clear_nils.
-
-    (* relate starting frame fr and fr_saved_and_tag *)
-    pose proof (frame_rel_mask_trans_combine _ _ _ _ _ Hfrel_fr_saved Hfrel_fr_saved_and_tag) as Hfrel_fr_and_fr_saved_and_tag.
-    simpl in Hfrel_fr_and_fr_saved_and_tag.
-
-    assert (frame_rel lmask fr fr_saved_and_tag) as Hfrel_lmask_saved_and_tag.
-    {
-      eapply frame_rel_mask_mono; [| exact Hfrel_fr_and_fr_saved_and_tag].
-      intros i [Hi_lo Hi_hi].
-      split.
-      + rewrite Hval_idxs_seq.
-        intro Hin. apply elem_of_seq in Hin. lia.
-      + unfold tag_idx. rewrite length_app. lia.
-    }
-    pose proof Hfrel_fr_and_fr_saved_and_tag as [_ ->].
-    iDestruct (labels_interp_mono _ _ _ _ fr_saved_and_tag _ _ _ _ with "Hlabels") as "Hlabels'"; first done.
-    {
-      instantiate (1 := (wlmask (fe_of_context F') (wl ++ wl_save ++ [prelude.W.T_i32]))).
-      intros i [Hi_lo Hi_hi].
-      simpl.
-      split.
-      + exact Hi_lo.
-      + rewrite -fe_of_context_labels.
-        rewrite !length_app. simpl.
-        subst fe.
-        lia.
-    }
-
-    assert (Forall2 (λ (i : prelude.W.localidx) (v : value), f_locs fr_saved_and_tag !! localimm i = Some v)
-      val_localidxs vs_payload) as Hfr_saved_and_tag_payload.
-    {
-      eapply forall2_lookup_same.
-      3: done.
-      - intros j Hneq. instantiate (1 := tag_idx) in Hneq.
-        destruct Hfrel_fr_saved_and_tag as [-> _]; done.
-      - subst val_idxs val_localidxs tag_idx.
-        rewrite length_app Nat.add_assoc.
-        apply map_seq_forall_localidx_neq.
-    }
-
-    iAssert
-      (frame_interp rti sr se L (wl ++ wl_save ++ [prelude.W.T_i32] ++ wl_case_1 ++ wl_case_2 ++ wl_case_3 ++ wlf) fr_saved_and_tag)
-      with "[Hframe_saved]" as "Hframe_saved_and_tag".
-    { admit. } (* TODO: Not really sure how to prove this. Definitely need helper lemma *)
-
-    (* Create defaults *)
-    iApply (cwp_seq with "[Hfr Hrun]").
-    {
-      eapply cwp_create_defaults in Hcreate_defaults as (_ & _ & _ & Hcreate_defaults).
-      iDestruct (Hcreate_defaults with "[$] [$] []") as "Hcreate_defaults".
-      {
-        by instantiate (1 := λ f vs, (⌜f = fr_saved_and_tag⌝ ∗ ⌜vs = (map default_of_value_type wl_ret)⌝)%I).
-      }
-      iApply "Hcreate_defaults".
-    }
-    iIntros (??) "[-> ->] Hfr Hrun".
-
-    (* Case analysis: Is tag 0 or 1 or 2? *)
-
-    apply lookup_lt_Some in Htag_type_lookup as Hi.
-    destruct tag as [| [|[|]]]; last done.
-
-    - (* Case: tag = 0 *)
-      (* -------- Case 1 -------- *)
-      rewrite (app_assoc (to_consts _)).
-      iApply (cwp_seq with "[-]").
-      {
-        iApply (compat_case_block_success with "[] [$] [$] [$] [$] [$] [$] [$] [$] [$]").
-        2: instantiate (1 := []).
-        all: clear_nils.
-        1, 2, 3, 4, 5, 6, 8, 9, 11, 13, 14: done.
-        4: iApply "Hsem_es1".
-        1: done.
-        1: by rewrite length_map.
-        by subst val_idxs.
-      }
-      iIntros (f_es_case_1 vs) "(_ & %Hlen_vs & %Hfrel_new & Hframe & %os & %θ' & Hos & Hvs & Hrt) Hfr Hrun".
-
-      (* -------- Case 2 -------- *)
-      rewrite (app_assoc (to_consts _)).
-      iApply (cwp_seq with "[Hfr Hrun]").
-      {
-        iApply (compat_case_block_fail with "[$] [$]").
-        2, 3, 4, 5, 6, 7, 8, 9, 10: done.
-        rewrite -Hsaved_and_tag.
-        destruct Hfrel_new as [Hmask _].
-        symmetry.
-        apply Hmask.
-        subst tag_idx fe.
-        unfold wlmask.
-        repeat rewrite length_app.
-        rewrite -fe_of_context_labels.
-        lias.
-      }
-      iIntros (??) "(-> & ->) Hfr Hrun".
-
-      (* -------- Case 3 -------- *)
-      iApply (cwp_wand with "[Hfr Hrun]").
-      {
-        iApply (compat_case_block_fail with "[$] [$]").
-        2, 3, 4, 5, 6, 8, 9, 10: done.
-        2: done.
-        rewrite -Hsaved_and_tag.
-        destruct Hfrel_new as [Hmask _].
-        symmetry.
-        apply Hmask.
-        subst tag_idx fe.
-        unfold wlmask.
-        repeat rewrite length_app.
-        rewrite -fe_of_context_labels.
-        lias.
-      }
-      iIntros (??) "(-> & ->)".
-      iFrame.
-      iPureIntro.
-      rewrite -fe_of_context_labels in Hfrel_new.
-      unfold lmask.
-      eapply frame_rel_trans.
-      + eapply frame_rel_mask_mono; [| exact Hfrel_lmask_saved_and_tag].
-        intros i [Hi_lo Hi_hi]. unfold lmask, wlmask. split; exact Hi_lo || exact Hi_hi.
-      + eapply frame_rel_wlmask_mono; [| exact Hfrel_new].
-        rewrite length_app. lia.
-
-    - (* Case: tag = 1 *)
-      (* -------- Case 1 -------- *)
-      rewrite (app_assoc (to_consts _)).
-      iApply (cwp_seq with "[Hfr Hrun]").
-      {
-        iApply (compat_case_block_fail with "[$] [$]").
-        7: by instantiate (1 := 1).
-        2: instantiate (1 := []).
-        1, 2, 3, 4, 5, 6, 7, 8: done.
-        by rewrite length_map.
-      }
-      iIntros (??) "(-> & ->) Hfr Hrun".
-
-      iDestruct (labels_interp_mono _ _ _ _ fr_saved_and_tag _ _ _ _ with "Hlabels") as "Hlabels'''"; first done.
-      {
-        instantiate (1 := (wlmask (fe_of_context F') (wl ++ wl_save ++ [prelude.W.T_i32] ++ wl_case_1))).
-        intros i [Hi_lo Hi_hi].
-        simpl.
-        split.
-        + exact Hi_lo.
-        + rewrite -fe_of_context_labels.
-          rewrite !length_app. simpl.
-          subst fe.
-          lia.
-      }
-
-      (* -------- Case 2 -------- *)
-      rewrite (app_assoc (to_consts _)).
-      iApply (cwp_seq with "[-]").
-      {
-        iApply (compat_case_block_success with "[] [$] [$] [$] [$] [$] [$] [$] [$] [$]").
-        1, 2, 3, 4, 5, 6, 8, 9, 11, 13, 14: done.
-        4: iApply "Hsem_es2".
-        1: done.
-        1: by rewrite length_map.
-        by subst val_idxs.
-      }
-      iIntros (f_es_case_2 vs) "(_ & %Hlen_vs & %Hfrel_new & Hframe & %os & %θ' & Hos & Hvs & Hrt) Hfr Hrun".
-
-      (* -------- Case 3 -------- *)
-      iApply (cwp_wand with "[Hfr Hrun]").
-      {
-        iApply (compat_case_block_fail with "[$] [$]").
-        2, 3, 4, 5, 6, 8, 9, 10: done.
-        2: done.
-        rewrite -Hsaved_and_tag.
-        destruct Hfrel_new as [Hmask _].
-        symmetry.
-        apply Hmask.
-        subst tag_idx fe.
-        unfold wlmask.
-        repeat rewrite length_app.
-        rewrite -fe_of_context_labels.
-        lias.
-      }
-      iIntros (??) "(-> & ->)".
-      iFrame.
-      iPureIntro.
-      rewrite -fe_of_context_labels in Hfrel_new.
-      unfold lmask.
-      eapply frame_rel_trans.
-      + eapply frame_rel_mask_mono; [| exact Hfrel_lmask_saved_and_tag].
-        intros i [Hi_lo Hi_hi]. unfold lmask, wlmask. split; exact Hi_lo || exact Hi_hi.
-      + eapply frame_rel_wlmask_mono; [| exact Hfrel_new].
-        rewrite length_app. lia.
-
-    - (* Case: tag = 2 *)
-      (* -------- Case 1 -------- *)
-      rewrite (app_assoc (to_consts _)).
-      iApply (cwp_seq with "[Hfr Hrun]").
-      {
-        iApply (compat_case_block_fail with "[$] [$]").
-        7: by instantiate (1 := 2).
-        2: instantiate (1 := []).
-        1, 2, 3, 4, 5, 6, 7, 8: done.
-        by rewrite length_map.
-      }
-      iIntros (??) "(-> & ->) Hfr Hrun".
-
-      (* -------- Case 2 -------- *)
-      rewrite (app_assoc (to_consts _)).
-      iApply (cwp_seq with "[Hfr Hrun]").
-      {
-        iApply (compat_case_block_fail with "[$] [$]").
-        7: by instantiate (1 := 2).
-        2: instantiate (1 := wl_case_1).
-        1, 2, 3, 4, 5, 6, 7, 8: done.
-        by rewrite length_map.
-      }
-      iIntros (??) "(-> & ->) Hfr Hrun".
-
-      iDestruct (labels_interp_mono _ _ _ _ fr_saved_and_tag _ _ _ _ with "Hlabels") as "Hlabels'''"; first done.
-      {
-        instantiate (1 := (wlmask (fe_of_context F') (wl ++ wl_save ++ [prelude.W.T_i32] ++ wl_case_1 ++ wl_case_2))).
-        intros i [Hi_lo Hi_hi].
-        simpl.
-        split.
-        + exact Hi_lo.
-        + rewrite -fe_of_context_labels.
-          rewrite !length_app. simpl.
-          subst fe.
-          lia.
-      }
-
-      (* -------- Case 3 -------- *)
-      iApply (cwp_wand with "[-]").
-      {
-        iApply (compat_case_block_success with "[] [$] [$] [$] [$] [$] [$] [$] [$] [$]").
-        1, 2, 3, 4, 5, 6, 8, 9, 11, 13, 14: done.
-        4: iApply "Hsem_es3".
-        1: done.
-        1: by rewrite length_map.
-        by subst val_idxs.
-      }
-      iIntros (f_es_case_3 vs) "(_ & %Hlen_vs & %Hfrel_new & Hframe & %os & %θ' & Hos & Hvs & Hrt)".
-      iFrame.
-      iPureIntro.
-      rewrite -fe_of_context_labels in Hfrel_new.
-      unfold lmask.
-      eapply frame_rel_trans.
-      + eapply frame_rel_mask_mono; [| exact Hfrel_lmask_saved_and_tag].
-        intros i [Hi_lo Hi_hi]. unfold lmask, wlmask. split; exact Hi_lo || exact Hi_hi.
-      + eapply frame_rel_wlmask_mono; [| exact Hfrel_new].
-        rewrite length_app. lia.
-  Admitted.
-
-
-  Lemma compile_cases_app fe ess1 ess2 :
-    (fix compile_cases fe ess := match ess with
-     | [] => [] | es :: ess' => mapM_ (compile_instr mr fe) es :: compile_cases fe ess'
-     end) fe (ess1 ++ ess2) =
-    (fix compile_cases fe ess := match ess with
-     | [] => [] | es :: ess' => mapM_ (compile_instr mr fe) es :: compile_cases fe ess'
-     end) fe ess1 ++
-    (fix compile_cases fe ess := match ess with
-     | [] => [] | es :: ess' => mapM_ (compile_instr mr fe) es :: compile_cases fe ess'
-     end) fe ess2.
-  Proof.
-    induction ess1; simpl; [done | by rewrite IHess1].
-  Qed.
 
   Lemma compat_case M F L L' wt wt' wtf wl wl' wlf es' ess τs τs' κ :
     let fe := fe_of_context F in
@@ -1407,6 +1636,7 @@ Proof.
     }
     assert (tag < Wasm_int.Int32.modulus)%Z as Htag_in_i32_bound.
     { rewrite Htyp_rep_len in Htag_size_bound. eapply Z.lt_le_trans; last done. by apply Nat2Z.inj_lt. }
+    assert (length τs = length ess) as Hess_typ_len; first by eapply List.Forall2_length.
 
     iDestruct (big_sepL2_length with "Hrvs") as "%Hlen".
     destruct vs as [|v_tag vs_payload]; first inversion Hlen.
@@ -1428,6 +1658,9 @@ Proof.
       (ess_pre & ess_rest & Hforall_pre & Hforall_rest & ->).
     apply Forall2_cons_inv_l in Hforall_rest as
       (es_tag & ess_post & Hforall_tag & Hforall_post & ->).
+    apply Forall2_length in Hforall_pre as Hess_pre_τs_pre.
+    apply Forall2_length in Hforall_post as Hess_post_τs_post.
+    clear Hforall_pre Hforall_post.
 
 
     (* save payload *)
@@ -1563,373 +1796,28 @@ Proof.
     rewrite separate1 in Hcg.
     apply run_codegen_case_blocks_blocks_app in Hcg as (wt_pre & wt_tag & wt_post & wl_pre & wl_tag & wl_post & es_pre & es_tag_cg & es_post & Hcg_pre & Hcg_tag & Hcg_post & -> & -> & ->).
 
-    (* (* Case blocks *) *)
-    (* cbv [map length seq zip Datatypes.uncurry] in Hcg. *)
-    (**)
-    (* clear_nils. *)
-    (**)
-    (* inv_cg_bind Hcg ?units ?wt ?wt ?wl ?wl ?es es_case_i Hcases Hret. *)
-    (* inv_cg_ret Hret; subst. *)
-    (**)
-    (* (* Case es_i *) *)
-    (* inv_cg_bind Hcases [] ?wt ?wt ?wl ?wl ?es es_rest Hcase_es_i Hrest. *)
-    (**)
-    (* inv_cg_bind Hcase_es_i ?pair ?wt ?wt ?wl ?wl ?es ?es Hcase_es_i Hcase_es_i_block. *)
-    (* destruct pair, u. *)
-    (* inv_cg_emit Hcase_es_i_block; subst. *)
-    (* apply run_codegen_capture in Hcase_es_i as [Hcase_es_i ->]. *)
-    (**)
-    (* inv_cg_bind Hcase_es_i [] ?wt ?wt ?wl ?wl ?es ?es Hget_tag Hcase_es_i. *)
-    (* inv_cg_emit Hget_tag; subst. *)
-    (**)
-    (* inv_cg_bind Hcase_es_i [] ?wt ?wt ?wl ?wl ?es ?es Htag0 Hcase_es_i. *)
-    (* inv_cg_emit Htag0; subst. *)
-    (**)
-    (* inv_cg_bind Hcase_es_i [] ?wt ?wt ?wl ?wl ?es ?es Hcompare_tag Hcase_es_i. *)
-    (* inv_cg_emit Hcompare_tag; subst. *)
-    (**)
-    (* inv_cg_bind Hcase_es_i [] ?wt ?wt ?wl ?wl ?es ?es Hbr_case Hcase_es_i. *)
-    (* inv_cg_emit Hbr_case; subst. *)
-    (**)
-    (* inv_cg_bind Hcase_es_i [] ?wt ?wt ?wl ?wl es_drop_i ?es Hdrop_consts_i Hcase_es_i. *)
-    (* apply run_codegen_drop_consts in Hdrop_consts_i as H. *)
-    (* destruct H as (_ & -> & -> & _). *)
-    (**)
-    (* inv_cg_bind Hcase_es_i ρ_casei ?wt ?wt ?wl ?wl ?es ?es Hlookup Hcase_es_i. *)
-    (* inv_cg_try_option Hlookup; subst. *)
-    (**)
-    (* inv_cg_bind Hcase_es_i case_i_sum_locals ?wt ?wt ?wl ?wl ?es ?es Hinject Hcase_es_i. *)
-    (* inv_cg_try_option Hinject; subst. *)
-    (**)
-    (* inv_cg_bind Hcase_es_i [] ?wt wt_case_i ?wl wl_case_i ?es es_case_i Hget_locals_i Hcase_es_i. *)
-    (* inv_cg_bind Hget_locals_i case_i_val_idxs ?wt wt_get_locals_i ?wl wl_get_locals_i ?es es_get_locals_i Hnths_error Hget_locals_i. *)
-    (* inv_cg_try_option Hnths_error; subst. *)
-    (**)
-    (* destruct (run_codegen_get_locals _ _ _ _ _ _ _ Hget_locals_i) as ([] & -> & ->). *)
-    (**)
-    (* (* clean up *) *)
-    (* subst WT WL. *)
-    (* clear_nils. *)
-    (* simplify_eq. *)
-    (**)
-    (**)
-    (* (* save payload *) *)
-    (* rewrite (app_assoc (e_tag ++ _)). *)
-    (* iApply (cwp_seq with "[Hfr Hrun]"). *)
-    (* { *)
-    (*   rewrite <- (app_assoc e_tag). *)
-    (*   instantiate (1 := λ fr' vs, ( *)
-    (*     ∃ val_idxs, *)
-    (*     ⌜vs = [VAL_int32 (Wasm_int.Int32.repr tag)]⌝ ∗ *)
-    (*     ⌜frame_rel (λ i, i ∉ val_idxs) fr fr'⌝ ∗ *)
-    (*     ⌜Forall2 (fun i v => f_locs fr' !! localimm i = Some v) val_localidxs vs_payload⌝ ∗ *)
-    (*     ⌜val_idxs = seq (fe_wlocal_offset fe + length wl) (length wl_save)⌝ ∗ *)
-    (*     ⌜val_localidxs = map prelude.W.Mk_localidx val_idxs⌝ *)
-    (*     )%I). *)
-    (*   iApply cwp_val_app; first done. *)
-    (*   eapply cwp_save_stack_w in Hsave; eauto. *)
-    (*   + destruct Hsave as (-> & -> & -> & Hsave). *)
-    (*     iApply (Hsave with "[$] [$]"). *)
-    (*     iIntros (f' [Hfsame Hfchanged]). *)
-    (*     unfold fvs_combine. *)
-    (*     auto. *)
-    (*   + admit. (* easy pure conseqeunce of value_interp and *)
-    (*   rep_values_interp, should be proved above the first wp_seq *)
-    (*   rule *) *)
-    (* } *)
-    (* iIntros (fr_saved w) "(%val_idxs & -> & %Hfrel_fr_saved & %Hsaved & %Hval_idxs_seq & %Hval_localidxs) Hfr Hrun". *)
-    (* iAssert *)
-    (* (frame_interp rti sr se L (wl ++ wl_save ++ [prelude.W.T_i32] ++ wl_case_i ++ wl2 ++ wlf) fr_saved) *)
-    (*   with "[Hframe]" as "Hframe_saved". *)
-    (* { admit. } (* TODO: Not really sure how to prove this. Definitely need helper lemma *) *)
-    (**)
-    (* edestruct (util.nths_error_exists val_localidxs case_i_val_idxs vs_payload case_i_sum_locals (Forall2_length _ _ _ Hsaved)) as [case_i_vs_payload Hnerr_payload_ci]; try done. *)
-    (**)
-    (* iDestruct (frame_interp_wl_interp with "Hframe_saved") as "%Hwl_saved"; first done. *)
-    (* pose proof (interp_wl_length _ _ _ Hwl_saved) as Hfr_saved_locs_len. *)
-    (**)
-    (* assert (tag_idx < length (f_locs fr_saved)) as Htag_in_fr_saved. *)
-    (* { *)
-    (*   subst tag_idx. *)
-    (*   simpl. *)
-    (*   eapply Nat.lt_le_trans; last done. *)
-    (*   - rewrite app_assoc. *)
-    (*     subst fe. *)
-    (*     instantiate (1 := F). *)
-    (*     repeat rewrite length_app. *)
-    (*     lias. *)
-    (* } *)
-    (**)
-    (* (* Store tag *) *)
-    (* rewrite (app_assoc (map _ _)). *)
-    (* iApply (cwp_seq with "[Hfr Hrun]"). *)
-    (* { *)
-    (*   instantiate (1 := λ fr' vs, ( *)
-    (*     ⌜vs = []⌝ ∗ *)
-    (*     ⌜frame_rel (λ j, j ≠ tag_idx) fr_saved fr'⌝ ∗ *)
-    (*     ⌜f_locs fr' !! tag_idx = Some (VAL_int32 (Wasm_int.Int32.repr tag))⌝ *)
-    (*     )%I). *)
-    (*   iApply (cwp_local_set with "[] [$] [$]"); first done. *)
-    (*   iSplit; first done. *)
-    (*   iSplit. *)
-    (*   - iPureIntro. *)
-    (*     split; last done. *)
-    (*     intros j Hneq. *)
-    (*     simpl. *)
-    (*     rewrite list_lookup_insert_ne; [reflexivity | lia]. *)
-    (*   - iSimpl. *)
-    (*     iPureIntro. *)
-    (*     rewrite list_lookup_insert_eq; try done. *)
-    (* } *)
-    (* iIntros (fr_saved_and_tag w) "(-> & %Hfrel_fr_saved_and_tag & %Hsaved_and_tag) Hfr Hrun". *)
-    (* clear_nils. *)
-    (**)
-    (* (* relate starting frame fr and fr_saved_and_tag *) *)
-    (* pose proof (frame_rel_mask_trans_combine _ _ _ _ _ Hfrel_fr_saved Hfrel_fr_saved_and_tag) as Hfrel_fr_and_fr_saved_and_tag. *)
-    (* simpl in Hfrel_fr_and_fr_saved_and_tag. *)
-    (**)
-    (* assert (frame_rel lmask fr fr_saved_and_tag) as Hfrel_lmask_saved_and_tag. *)
-    (* { *)
-    (*   eapply frame_rel_mask_mono; [| exact Hfrel_fr_and_fr_saved_and_tag]. *)
-    (*   intros i [Hi_lo Hi_hi]. *)
-    (*   split. *)
-    (*   + rewrite Hval_idxs_seq. *)
-    (*     intro Hin. apply elem_of_seq in Hin. lia. *)
-    (*   + unfold tag_idx. rewrite length_app. lia. *)
-    (* } *)
-    (* pose proof Hfrel_fr_and_fr_saved_and_tag as [_ ->]. *)
-    (* iDestruct (labels_interp_mono _ _ _ _ fr_saved_and_tag _ _ _ _ with "Hlabels") as "Hlabels'"; first done. *)
-    (* { *)
-    (*   instantiate (1 := (wlmask (fe_of_context F') (wl ++ wl_save ++ [prelude.W.T_i32]))). *)
-    (*   intros i [Hi_lo Hi_hi]. *)
-    (*   simpl. *)
-    (*   split. *)
-    (*   + exact Hi_lo. *)
-    (*   + rewrite -fe_of_context_labels. *)
-    (*     rewrite !length_app. simpl. *)
-    (*     subst fe. *)
-    (*     lia. *)
-    (* } *)
-    (**)
-    (* assert (Forall2 (λ (i : prelude.W.localidx) (v : value), f_locs fr_saved_and_tag !! localimm i = Some v) *)
-    (*   val_localidxs vs_payload) as Hfr_saved_and_tag_payload. *)
-    (* { *)
-    (*   eapply forall2_lookup_same. *)
-    (*   3: done. *)
-    (*   - intros j Hneq. instantiate (1 := tag_idx) in Hneq. *)
-    (*     destruct Hfrel_fr_saved_and_tag as [-> _]; done. *)
-    (*   - subst val_idxs val_localidxs tag_idx. *)
-    (*     rewrite length_app Nat.add_assoc. *)
-    (*     apply map_seq_forall_localidx_neq. *)
-    (* } *)
-    (**)
-    (* iAssert *)
-    (* (frame_interp rti sr se L (wl ++ wl_save ++ [prelude.W.T_i32] ++ wl_case_i ++ wl2 ++ wlf) fr_saved_and_tag) *)
-    (*   with "[Hframe_saved]" as "Hframe_saved_and_tag". *)
-    (* { admit. } (* TODO: Not really sure how to prove this. Definitely need helper lemma *) *)
-    (**)
-    (* (* Create defaults *) *)
-    (* iApply (cwp_seq with "[Hfr Hrun]"). *)
-    (* { *)
-    (*   eapply cwp_create_defaults in Hcreate_defaults as (_ & _ & _ & Hcreate_defaults). *)
-    (*   iDestruct (Hcreate_defaults with "[$] [$] []") as "Hcreate_defaults". *)
-    (*   { *)
-    (*     by instantiate (1 := λ f vs, (⌜f = fr_saved_and_tag⌝ ∗ ⌜vs = (map default_of_value_type wl_ret)⌝)%I). *)
-    (*   } *)
-    (*   iApply "Hcreate_defaults". *)
-    (* } *)
-    (* iIntros (??) "[-> ->] Hfr Hrun". *)
-    (**)
-    (* (* Case analysis: Is tag 0  *) *)
-    (**)
-    (* apply lookup_lt_Some in Htag_type_lookup as Hi. *)
-    (* destruct tag as [| [|[|]]]; last done. *)
-    (**)
-    (* - (* Case: tag = 0 *) *)
-    (*   (* -------- Case 1 -------- *) *)
-    (*   rewrite (app_assoc (to_consts _)). *)
-    (*   iApply (cwp_seq with "[-]"). *)
-    (*   { *)
-    (*     iApply (compat_case_block_success with "[] [$] [$] [$] [$] [$] [$] [$] [$] [$]"). *)
-    (*     2: instantiate (1 := []). *)
-    (*     all: clear_nils. *)
-    (*     1, 2, 3, 4, 5, 6, 8, 9, 11, 13, 14: done. *)
-    (*     4: iApply "Hsem_es1". *)
-    (*     1: done. *)
-    (*     1: by rewrite length_map. *)
-    (*     by subst val_idxs. *)
-    (*   } *)
-    (*   iIntros (f_es_case_1 vs) "(_ & %Hlen_vs & %Hfrel_new & Hframe & %os & %θ' & Hos & Hvs & Hrt) Hfr Hrun". *)
-    (**)
-    (*   (* -------- Case 2 -------- *) *)
-    (*   rewrite (app_assoc (to_consts _)). *)
-    (*   iApply (cwp_seq with "[Hfr Hrun]"). *)
-    (*   { *)
-    (*     iApply (compat_case_block_fail with "[$] [$]"). *)
-    (*     2, 3, 4, 5, 6, 7, 8, 9, 10: done. *)
-    (*     rewrite -Hsaved_and_tag. *)
-    (*     destruct Hfrel_new as [Hmask _]. *)
-    (*     symmetry. *)
-    (*     apply Hmask. *)
-    (*     subst tag_idx fe. *)
-    (*     unfold wlmask. *)
-    (*     repeat rewrite length_app. *)
-    (*     rewrite -fe_of_context_labels. *)
-    (*     lias. *)
-    (*   } *)
-    (*   iIntros (??) "(-> & ->) Hfr Hrun". *)
-    (**)
-    (*   (* -------- Case 3 -------- *) *)
-    (*   iApply (cwp_wand with "[Hfr Hrun]"). *)
-    (*   { *)
-    (*     iApply (compat_case_block_fail with "[$] [$]"). *)
-    (*     2, 3, 4, 5, 6, 8, 9, 10: done. *)
-    (*     2: done. *)
-    (*     rewrite -Hsaved_and_tag. *)
-    (*     destruct Hfrel_new as [Hmask _]. *)
-    (*     symmetry. *)
-    (*     apply Hmask. *)
-    (*     subst tag_idx fe. *)
-    (*     unfold wlmask. *)
-    (*     repeat rewrite length_app. *)
-    (*     rewrite -fe_of_context_labels. *)
-    (*     lias. *)
-    (*   } *)
-    (*   iIntros (??) "(-> & ->)". *)
-    (*   iFrame. *)
-    (*   iPureIntro. *)
-    (*   rewrite -fe_of_context_labels in Hfrel_new. *)
-    (*   unfold lmask. *)
-    (*   eapply frame_rel_trans. *)
-    (*   + eapply frame_rel_mask_mono; [| exact Hfrel_lmask_saved_and_tag]. *)
-    (*     intros i [Hi_lo Hi_hi]. unfold lmask, wlmask. split; exact Hi_lo || exact Hi_hi. *)
-    (*   + eapply frame_rel_wlmask_mono; [| exact Hfrel_new]. *)
-    (*     rewrite length_app. lia. *)
-    (**)
-    (* - (* Case: tag = 1 *) *)
-    (*   (* -------- Case 1 -------- *) *)
-    (*   rewrite (app_assoc (to_consts _)). *)
-    (*   iApply (cwp_seq with "[Hfr Hrun]"). *)
-    (*   { *)
-    (*     iApply (compat_case_block_fail with "[$] [$]"). *)
-    (*     7: by instantiate (1 := 1). *)
-    (*     2: instantiate (1 := []). *)
-    (*     1, 2, 3, 4, 5, 6, 7, 8: done. *)
-    (*     by rewrite length_map. *)
-    (*   } *)
-    (*   iIntros (??) "(-> & ->) Hfr Hrun". *)
-    (**)
-    (*   iDestruct (labels_interp_mono _ _ _ _ fr_saved_and_tag _ _ _ _ with "Hlabels") as "Hlabels'''"; first done. *)
-    (*   { *)
-    (*     instantiate (1 := (wlmask (fe_of_context F') (wl ++ wl_save ++ [prelude.W.T_i32] ++ wl_case_1))). *)
-    (*     intros i [Hi_lo Hi_hi]. *)
-    (*     simpl. *)
-    (*     split. *)
-    (*     + exact Hi_lo. *)
-    (*     + rewrite -fe_of_context_labels. *)
-    (*       rewrite !length_app. simpl. *)
-    (*       subst fe. *)
-    (*       lia. *)
-    (*   } *)
-    (**)
-    (*   (* -------- Case 2 -------- *) *)
-    (*   rewrite (app_assoc (to_consts _)). *)
-    (*   iApply (cwp_seq with "[-]"). *)
-    (*   { *)
-    (*     iApply (compat_case_block_success with "[] [$] [$] [$] [$] [$] [$] [$] [$] [$]"). *)
-    (*     1, 2, 3, 4, 5, 6, 8, 9, 11, 13, 14: done. *)
-    (*     4: iApply "Hsem_es2". *)
-    (*     1: done. *)
-    (*     1: by rewrite length_map. *)
-    (*     by subst val_idxs. *)
-    (*   } *)
-    (*   iIntros (f_es_case_2 vs) "(_ & %Hlen_vs & %Hfrel_new & Hframe & %os & %θ' & Hos & Hvs & Hrt) Hfr Hrun". *)
-    (**)
-    (*   (* -------- Case 3 -------- *) *)
-    (*   iApply (cwp_wand with "[Hfr Hrun]"). *)
-    (*   { *)
-    (*     iApply (compat_case_block_fail with "[$] [$]"). *)
-    (*     2, 3, 4, 5, 6, 8, 9, 10: done. *)
-    (*     2: done. *)
-    (*     rewrite -Hsaved_and_tag. *)
-    (*     destruct Hfrel_new as [Hmask _]. *)
-    (*     symmetry. *)
-    (*     apply Hmask. *)
-    (*     subst tag_idx fe. *)
-    (*     unfold wlmask. *)
-    (*     repeat rewrite length_app. *)
-    (*     rewrite -fe_of_context_labels. *)
-    (*     lias. *)
-    (*   } *)
-    (*   iIntros (??) "(-> & ->)". *)
-    (*   iFrame. *)
-    (*   iPureIntro. *)
-    (*   rewrite -fe_of_context_labels in Hfrel_new. *)
-    (*   unfold lmask. *)
-    (*   eapply frame_rel_trans. *)
-    (*   + eapply frame_rel_mask_mono; [| exact Hfrel_lmask_saved_and_tag]. *)
-    (*     intros i [Hi_lo Hi_hi]. unfold lmask, wlmask. split; exact Hi_lo || exact Hi_hi. *)
-    (*   + eapply frame_rel_wlmask_mono; [| exact Hfrel_new]. *)
-    (*     rewrite length_app. lia. *)
-    (**)
-    (* - (* Case: tag = 2 *) *)
-    (*   (* -------- Case 1 -------- *) *)
-    (*   rewrite (app_assoc (to_consts _)). *)
-    (*   iApply (cwp_seq with "[Hfr Hrun]"). *)
-    (*   { *)
-    (*     iApply (compat_case_block_fail with "[$] [$]"). *)
-    (*     7: by instantiate (1 := 2). *)
-    (*     2: instantiate (1 := []). *)
-    (*     1, 2, 3, 4, 5, 6, 7, 8: done. *)
-    (*     by rewrite length_map. *)
-    (*   } *)
-    (*   iIntros (??) "(-> & ->) Hfr Hrun". *)
-    (**)
-    (*   (* -------- Case 2 -------- *) *)
-    (*   rewrite (app_assoc (to_consts _)). *)
-    (*   iApply (cwp_seq with "[Hfr Hrun]"). *)
-    (*   { *)
-    (*     iApply (compat_case_block_fail with "[$] [$]"). *)
-    (*     7: by instantiate (1 := 2). *)
-    (*     2: instantiate (1 := wl_case_1). *)
-    (*     1, 2, 3, 4, 5, 6, 7, 8: done. *)
-    (*     by rewrite length_map. *)
-    (*   } *)
-    (*   iIntros (??) "(-> & ->) Hfr Hrun". *)
-    (**)
-    (*   iDestruct (labels_interp_mono _ _ _ _ fr_saved_and_tag _ _ _ _ with "Hlabels") as "Hlabels'''"; first done. *)
-    (*   { *)
-    (*     instantiate (1 := (wlmask (fe_of_context F') (wl ++ wl_save ++ [prelude.W.T_i32] ++ wl_case_1 ++ wl_case_2))). *)
-    (*     intros i [Hi_lo Hi_hi]. *)
-    (*     simpl. *)
-    (*     split. *)
-    (*     + exact Hi_lo. *)
-    (*     + rewrite -fe_of_context_labels. *)
-    (*       rewrite !length_app. simpl. *)
-    (*       subst fe. *)
-    (*       lia. *)
-    (*   } *)
-    (**)
-    (*   (* -------- Case 3 -------- *) *)
-    (*   iApply (cwp_wand with "[-]"). *)
-    (*   { *)
-    (*     iApply (compat_case_block_success with "[] [$] [$] [$] [$] [$] [$] [$] [$] [$]"). *)
-    (*     1, 2, 3, 4, 5, 6, 8, 9, 11, 13, 14: done. *)
-    (*     4: iApply "Hsem_es3". *)
-    (*     1: done. *)
-    (*     1: by rewrite length_map. *)
-    (*     by subst val_idxs. *)
-    (*   } *)
-    (*   iIntros (f_es_case_3 vs) "(_ & %Hlen_vs & %Hfrel_new & Hframe & %os & %θ' & Hos & Hvs & Hrt)". *)
-    (*   iFrame. *)
-    (*   iPureIntro. *)
-    (*   rewrite -fe_of_context_labels in Hfrel_new. *)
-    (*   unfold lmask. *)
-    (*   eapply frame_rel_trans. *)
-    (*   + eapply frame_rel_mask_mono; [| exact Hfrel_lmask_saved_and_tag]. *)
-    (*     intros i [Hi_lo Hi_hi]. unfold lmask, wlmask. split; exact Hi_lo || exact Hi_hi. *)
-    (*   + eapply frame_rel_wlmask_mono; [| exact Hfrel_new]. *)
-    (*     rewrite length_app. lia. *)
+    replace (length (map _ _)) with (length ess_pre) in Hcg_tag, Hcg_post.
+    2: {
+      rewrite length_map.
+      apply compile_cases_length.
+    }
+    rewrite Nat.add_0_l in Hcg_tag, Hcg_post.
+
+
+    iEval (rewrite app_assoc).
+    iApply (cwp_seq with "[Hfr Hrun]").
+    {
+      iApply (compat_case_blocks_fail F (wt ++ wt_save) wt_pre tag_idx tag
+      wl_ret (wl ++ wl_save ++ [prelude.W.T_i32]) wl_pre
+      ρs_sum val_localidxs (map default_of_value_type wl_ret)
+      ess_pre es_pre 0 fr_saved_and_tag B R τ_res with "[$] [$]").
+      1: right; rewrite Nat.add_0_l; lia.
+      1, 2, 3, 4, 7: done.
+      1: lia.
+      by rewrite length_map.
+    }
+    iIntros (?fr w) "(-> & ->) Hfr Hrun".
+
   Admitted.
 
 End case.
